finish top loop of BFS

Pair_Graph/BFS_2.thy
@@ -1,6 +1,43 @@
 theory BFS_2
-  imports Pair_Graph_Specs "HOL-Eisbach.Eisbach_Tools"
+  imports Pair_Graph_Specs "HOL-Eisbach.Eisbach_Tools" "Dist"
 begin
+                                          
+lemma list_suffix_disjoint: "\<lbrakk>set xs \<inter> s \<noteq> {}; last xs \<notin> s\<rbrakk> \<Longrightarrow> \<exists>xs1 x xs2. xs = xs1 @ x # xs2 \<and> x \<in> s \<and> set xs2 \<inter> s = {}"
+proof(induction xs)
+  case Nil
+  then show ?case
+    by auto
+next
+  case (Cons a xs)
+  show ?case
+  proof(cases "set xs \<inter> s = {}")
+    case xs_disj_s: True
+    show ?thesis
+    proof(cases "xs = []")
+      case xs_neq_Nil: False
+      then have "a # xs = [] @ a # xs \<and> a \<in> s \<and> set xs \<inter> s = {}"
+        using Cons xs_disj_s
+        by auto
+      then show ?thesis 
+        by metis
+    qed (insert Cons, auto)
+  next
+    case xs_not_disj_s: False
+    then show ?thesis
+    proof(cases "xs = []")
+      case xs_neq_Nil: False
+      then have "\<exists>xs1 x xs2. xs = xs1 @ x # xs2 \<and> x \<in> s \<and> set xs2 \<inter> s = {}"
+        using Cons xs_not_disj_s
+        by (auto intro!: Cons )
+      then obtain xs1 x xs2 where "xs = xs1 @ x # xs2 \<and> x \<in> s \<and> set xs2 \<inter> s = {}"
+        by auto
+      hence "a # xs = (a # xs1) @ x # xs2 \<and> x \<in> s \<and> set xs2 \<inter> s = {}"
+        by auto
+      thus ?thesis
+        by metis
+    qed (insert Cons, auto)
+  qed
+qed
 
 datatype 'a tree = Leaf | Node "'a tree" 'a "'a tree"
 
@@ -108,25 +145,33 @@ locale BFS =
   
 for lookup :: "'adj \<Rightarrow> 'ver \<Rightarrow> 'neighb option" +
 
-fixes  G::"'adj" and expand_tree::"'adj \<Rightarrow> 'neighb \<Rightarrow> 'neighb \<Rightarrow> 'adj" and
+fixes  
+srcs::"'neighb" and
+G::"'adj" and expand_tree::"'adj \<Rightarrow> 'neighb \<Rightarrow> 'neighb \<Rightarrow> 'adj" and
 next_frontier::"'neighb \<Rightarrow> 'neighb \<Rightarrow> 'neighb" 
 
 
 assumes
    graph_inv[simp]:
      "Graph.graph_inv G" and
+   srcs_nempty[simp]:
+     "t_set srcs \<noteq> {}" and
    expand_tree[simp]:
-     "\<lbrakk>Graph.graph_inv BFS_tree; neighb_inv frontier; neighb_inv vis\<rbrakk> \<Longrightarrow> Graph.graph_inv (expand_tree BFS_tree frontier vis)"
+     "\<lbrakk>Graph.graph_inv BFS_tree; neighb_inv frontier; neighb_inv vis\<rbrakk> \<Longrightarrow> 
+       Graph.graph_inv (expand_tree BFS_tree frontier vis)"
      "\<lbrakk>Graph.graph_inv BFS_tree; neighb_inv frontier; neighb_inv vis\<rbrakk> \<Longrightarrow>
         Graph.digraph_abs (expand_tree BFS_tree frontier vis) = 
-         (Graph.digraph_abs BFS_tree) \<union> {(u,v) | u v. u \<in> t_set (frontier) \<and> v \<in> (Pair_Graph.neighbourhood (Graph.digraph_abs G) u - t_set vis)}" and
+         (Graph.digraph_abs BFS_tree) \<union> 
+         {(u,v) | u v. u \<in> t_set (frontier) \<and> 
+                       v \<in> (Pair_Graph.neighbourhood (Graph.digraph_abs G) u -
+                       t_set vis)}" and
    next_frontier[simp]:
     "\<lbrakk>neighb_inv frontier; neighb_inv vis\<rbrakk> \<Longrightarrow>  neighb_inv (next_frontier frontier vis)"
     "\<lbrakk>neighb_inv frontier; neighb_inv vis\<rbrakk> \<Longrightarrow>
        t_set (next_frontier frontier vis) =
-         (\<Union> {Pair_Graph.neighbourhood (Graph.digraph_abs G) u | u . u \<in> t_set frontier}) - t_set vis"
-    
-
+         (\<Union> {Pair_Graph.neighbourhood (Graph.digraph_abs G) u | u . u \<in> t_set frontier}) - t_set vis" and
+   finite_neighb:
+     "finite (Pair_Graph.neighbourhood (Graph.digraph_abs G) u)"
 begin
 
 abbreviation "neighbourhood' \<equiv> Graph.neighbourhood G" 
@@ -195,7 +240,7 @@ lemma BFS_ret_1_condsI[call_cond_intros]:
   "\<lbrakk>current bfs_state = \<emptyset>\<^sub>N\<rbrakk> \<Longrightarrow> BFS_ret_1_conds bfs_state"
   by(auto simp: BFS_ret_1_conds_def split: list.splits option.splits if_splits)
 
-abbreviation "BFS_ret1 dfs_state \<equiv> dfs_state"
+abbreviation "BFS_ret1 bfs_state \<equiv> bfs_state"
 
 lemma BFS_cases:
   assumes "BFS_call_1_conds bfs_state \<Longrightarrow> P"
@@ -235,24 +280,36 @@ lemma BFS_induct:
 
 definition "invar_1 bfs_state \<equiv>
               neighb_inv (visited bfs_state) \<and> neighb_inv (current bfs_state) \<and>
-              Graph.graph_inv (parents bfs_state)"
+              Graph.graph_inv (parents bfs_state) \<and> 
+              finite (t_set (current bfs_state)) \<and> finite (t_set (visited bfs_state))"
 
 lemma invar_1_props[elim]: 
   "invar_1 bfs_state \<Longrightarrow> 
   (\<lbrakk>neighb_inv (visited bfs_state) ; neighb_inv (current bfs_state) ;
-    Graph.graph_inv (parents bfs_state)\<rbrakk> \<Longrightarrow> P)
+    Graph.graph_inv (parents bfs_state); 
+    finite (t_set (current bfs_state)); finite (t_set (visited bfs_state))\<rbrakk> \<Longrightarrow> P)
      \<Longrightarrow> P"
   by (auto simp: invar_1_def)
 
 lemma invar_1_intro[invar_props_intros]:
   "\<lbrakk>neighb_inv (visited bfs_state); neighb_inv (current bfs_state);
-    Graph.graph_inv (parents bfs_state)\<rbrakk> 
+    Graph.graph_inv (parents bfs_state);
+    finite (t_set (current bfs_state)); finite (t_set (visited bfs_state))\<rbrakk> 
     \<Longrightarrow> invar_1 bfs_state"
   by (auto simp: invar_1_def)
 
+lemma finite_simp:
+   "{(u,v). u \<in> front \<and> v \<in> (Pair_Graph.neighbourhood (Graph.digraph_abs G) u) \<and> v \<notin> vis} = 
+       {(u,v). u \<in> front} \<inter> {(u,v). v \<in> (Pair_Graph.neighbourhood (Graph.digraph_abs G) u)} - {(u,v) . v \<in> vis}"
+   "finite {(u, v)| v . v \<in> (s u)} = finite (s u)"
+  using finite_image_iff[where f = snd and A = "{(u, v) |v. v \<in> s u}"]
+  by (auto simp: inj_on_def image_def)
+  
 lemma invar_1_holds_upd1[invar_holds_intros]:
   "\<lbrakk>BFS_call_1_conds bfs_state; invar_1 bfs_state\<rbrakk> \<Longrightarrow> invar_1 (BFS_upd1 bfs_state)"
-  by(auto elim!: call_cond_elims simp: Let_def BFS_upd1_def BFS_call_1_conds_def intro!: invar_props_intros invarI)
+  using finite_neighb
+  by(auto elim!: invar_1_props call_cond_elims simp: Let_def BFS_upd1_def BFS_call_1_conds_def intro!: invar_props_intros invarI)+
+
 
 lemma invar_1_holds_4[invar_holds_intros]:
   "\<lbrakk>BFS_ret_1_conds bfs_state; invar_1 bfs_state\<rbrakk> \<Longrightarrow> invar_1 (BFS_ret1 bfs_state)"
@@ -261,37 +318,34 @@ lemma invar_1_holds_4[invar_holds_intros]:
 definition "invar_2 bfs_state \<equiv> 
   Graph.digraph_abs (parents bfs_state) \<subseteq> Graph.digraph_abs G \<and> 
   t_set (current bfs_state) \<subseteq> dVs (Graph.digraph_abs G) \<and> 
-  dVs (Graph.digraph_abs (parents bfs_state)) \<subseteq> t_set (visited bfs_state) \<and>
-  t_set (current bfs_state) \<subseteq> t_set (visited bfs_state)"
+  dVs (Graph.digraph_abs (parents bfs_state)) = t_set (visited bfs_state) \<and>
+  t_set (current bfs_state) \<subseteq> dVs (Graph.digraph_abs (parents bfs_state)) \<and>
+  t_set srcs \<subseteq> t_set (visited bfs_state)"
 
 lemma invar_2_props[elim]: 
   "invar_2 bfs_state \<Longrightarrow> 
   (\<lbrakk>Graph.digraph_abs (parents bfs_state) \<subseteq> Graph.digraph_abs G;
     t_set (current bfs_state) \<subseteq> dVs (Graph.digraph_abs G);
-    dVs (Graph.digraph_abs (parents bfs_state)) \<subseteq> t_set (visited bfs_state);
-    t_set (current bfs_state) \<subseteq> t_set (visited bfs_state)\<rbrakk> \<Longrightarrow> P)
+    dVs (Graph.digraph_abs (parents bfs_state)) = t_set (visited bfs_state);
+    t_set (current bfs_state) \<subseteq> dVs (Graph.digraph_abs (parents bfs_state));
+    t_set srcs \<subseteq> t_set (visited bfs_state)\<rbrakk> \<Longrightarrow> P)
      \<Longrightarrow> P"
   by (auto simp: invar_2_def)
 
 lemma invar_2_intro[invar_props_intros]:
    "\<lbrakk>Graph.digraph_abs (parents bfs_state) \<subseteq> Graph.digraph_abs G;
      t_set (current bfs_state) \<subseteq> dVs (Graph.digraph_abs G);
-     dVs (Graph.digraph_abs (parents bfs_state)) \<subseteq> t_set (visited bfs_state);
-     t_set (current bfs_state) \<subseteq> t_set (visited bfs_state)\<rbrakk>
+     dVs (Graph.digraph_abs (parents bfs_state)) = t_set (visited bfs_state);
+     t_set (current bfs_state) \<subseteq> dVs (Graph.digraph_abs (parents bfs_state));
+     t_set srcs \<subseteq> t_set (visited bfs_state)\<rbrakk>
      \<Longrightarrow> invar_2 bfs_state"
   by (auto simp: invar_2_def)
 
 lemma invar_2_holds_upd1[invar_holds_intros]: 
   "\<lbrakk>BFS_call_1_conds bfs_state; invar_1 bfs_state; invar_2 bfs_state\<rbrakk> \<Longrightarrow> invar_2 (BFS_upd1 bfs_state)"
   apply(auto elim!: call_cond_elims invar_1_props invar_2_props intro!: invar_props_intros simp: BFS_upd1_def Let_def)
-
-  apply(auto elim!: call_cond_elims invar_1_props invar_2_props intro!: invar_props_intros simp: BFS_upd1_def dVs_def)
-
-
-  apply blast
-  apply blast
+  apply(auto simp: dVs_def)
   done
-
 
 lemma invar_2_holds_4[invar_holds_intros]:
   "\<lbrakk>BFS_ret_1_conds bfs_state; invar_2 bfs_state\<rbrakk> \<Longrightarrow> invar_2 (BFS_ret1 bfs_state)"
@@ -308,75 +362,1120 @@ proof(induction rule: BFS_induct[OF assms(1)])
     by (auto intro!: IH(2-) intro: invar_holds_intros  simp: BFS_simps[OF IH(1)])
 qed
 
+\<comment> \<open>This is invar\_100 on the board\<close>
 
-definition "invar_3 bfs_state \<equiv> 
-  (\<forall>v \<in> (dVs (Graph.digraph_abs (parents bfs_state))).
-    \<forall>u. (v \<rightarrow>\<^sup>*\<^bsub>Graph.digraph_abs G\<^esub> u) \<longrightarrow> 
-      ((v \<rightarrow>\<^sup>*\<^bsub>Graph.digraph_abs (parents bfs_state)\<^esub> u) 
-       \<or> (\<exists>w\<in>t_set (current bfs_state). (v \<rightarrow>\<^sup>*\<^bsub>Graph.digraph_abs (parents bfs_state)\<^esub> w) \<and> (w \<rightarrow>\<^sup>*\<^bsub>Graph.digraph_abs G\<^esub> u))))"
+definition "invar_3_1 bfs_state \<equiv> 
+  (\<forall>v\<in>t_set (current bfs_state). \<forall>u. u \<in> t_set (current bfs_state) \<longleftrightarrow> 
+      distance_set (Graph.digraph_abs G) (t_set srcs) v =
+                           distance_set (Graph.digraph_abs G) (t_set srcs) u)"
 
-lemma invar_3_props[elim]: 
-  "invar_3 bfs_state \<Longrightarrow> 
-  \<lbrakk>\<lbrakk>\<lbrakk>v \<in> (dVs (Graph.digraph_abs (parents bfs_state))); (v \<rightarrow>\<^sup>*\<^bsub>Graph.digraph_abs G\<^esub> u)\<rbrakk> \<Longrightarrow>
-          (v \<rightarrow>\<^sup>*\<^bsub>Graph.digraph_abs (parents bfs_state)\<^esub> u)\<rbrakk>
-           \<Longrightarrow> P;
-   \<lbrakk>\<lbrakk>v \<in> (dVs (Graph.digraph_abs (parents bfs_state))); (v \<rightarrow>\<^sup>*\<^bsub>Graph.digraph_abs G\<^esub> u)\<rbrakk> \<Longrightarrow>
-           (\<exists>w\<in>t_set (current bfs_state). (v \<rightarrow>\<^sup>*\<^bsub>Graph.digraph_abs (parents bfs_state)\<^esub> w) \<and> (w \<rightarrow>\<^sup>*\<^bsub>Graph.digraph_abs G\<^esub> u))\<rbrakk>
-           \<Longrightarrow> P\<rbrakk>
+lemma invar_3_1_props[elim]: 
+  "invar_3_1 bfs_state \<Longrightarrow>
+  (\<lbrakk>\<lbrakk>v \<in> t_set (current bfs_state); u \<in> t_set (current bfs_state)\<rbrakk> \<Longrightarrow>
+            distance_set (Graph.digraph_abs G) (t_set srcs) v =
+                 distance_set (Graph.digraph_abs G) (t_set srcs) u;
+    \<lbrakk>v \<in> t_set (current bfs_state);
+            distance_set (Graph.digraph_abs G) (t_set srcs) v = 
+              distance_set (Graph.digraph_abs G) (t_set srcs) u\<rbrakk> \<Longrightarrow>
+            u \<in> t_set (current bfs_state)\<rbrakk> \<Longrightarrow> P)
      \<Longrightarrow> P"
-  by (auto simp: invar_3_def)
+  unfolding invar_3_1_def
+  by blast
 
-lemma invar_3_intro[invar_props_intros]:
-   "(\<And>v u. \<lbrakk>v \<in> (dVs (Graph.digraph_abs (parents bfs_state))); (v \<rightarrow>\<^sup>*\<^bsub>Graph.digraph_abs G\<^esub> u)\<rbrakk> \<Longrightarrow>
-       (v \<rightarrow>\<^sup>*\<^bsub>Graph.digraph_abs (parents bfs_state)\<^esub> u) \<or>
-       (\<exists>w\<in>t_set (current bfs_state). (v \<rightarrow>\<^sup>*\<^bsub>Graph.digraph_abs (parents bfs_state)\<^esub> w) \<and> (w \<rightarrow>\<^sup>*\<^bsub>Graph.digraph_abs G\<^esub> u)))
-    \<Longrightarrow> invar_3 bfs_state"
-  by (auto simp: invar_3_def)
+lemma invar_3_1_intro[invar_props_intros]:
+   "\<lbrakk>\<And>u v. \<lbrakk>v \<in> t_set (current bfs_state); u \<in> t_set (current bfs_state)\<rbrakk> \<Longrightarrow>
+            distance_set (Graph.digraph_abs G) (t_set srcs) v =
+                           distance_set (Graph.digraph_abs G) (t_set srcs) u;
+     \<And>u v. \<lbrakk>v \<in> t_set (current bfs_state); distance_set (Graph.digraph_abs G) (t_set srcs) v =
+                 distance_set (Graph.digraph_abs G) (t_set srcs) u\<rbrakk> \<Longrightarrow>
+            u \<in> t_set (current bfs_state)\<rbrakk>
+    \<Longrightarrow> invar_3_1 bfs_state"
+  unfolding invar_3_1_def
+  by blast
 
-lemma invar_3_holds_upd1[invar_holds_intros]: 
-  assumes "BFS_call_1_conds bfs_state" "invar_1 bfs_state" "invar_2 bfs_state" "invar_3 bfs_state"
-  shows "invar_3 (BFS_upd1 bfs_state)"
-proof(rule invar_props_intros, goal_cases)
-  case (1 v u)
-  then show ?case 
-    using assms
-  proof(elim invar_3_props[where u = u and v = v], goal_cases)
-    case 1
-    find_theorems dVs "_\<union>_"
-    from \<open>invar_1 bfs_state\<close> \<open>invar_2 bfs_state\<close>
-    have "dVs (Graph.digraph_abs (parents (BFS_upd1 bfs_state))) \<subseteq>
-            dVs (Graph.digraph_abs (parents bfs_state)) \<union> {v | u v. u \<in> t_set (current bfs_state) \<and> v \<in> Pair_Graph.neighbourhood (Graph.digraph_abs G) u}"
-      apply (auto simp: BFS_upd1_def Let_def elim!: in_dVsE invar_1_props invar_2_props)
+\<comment> \<open>This is equivalent to 200 on the board, except that I changed tree to G\<close>
 
-      apply (auto simp: BFS_upd1_def Let_def dVs_def elim!: in_dVsE invar_1_props invar_2_props)
-      sledgehammer
-      apply (metis insertI1)
+definition "invar_3_1' bfs_state \<equiv> 
+  (\<forall>v\<in>t_set (current bfs_state). \<forall>u. u \<in> t_set (current bfs_state) \<longleftrightarrow> 
+      distance_set (Graph.digraph_abs (parents bfs_state)) (t_set srcs) v =
+                           distance_set (Graph.digraph_abs (parents bfs_state)) (t_set srcs) u)"
+
+lemma invar_3_1'_props[elim]: 
+  "invar_3_1' bfs_state \<Longrightarrow>
+  (\<lbrakk>\<lbrakk>v \<in> t_set (current bfs_state); u \<in> t_set (current bfs_state)\<rbrakk> \<Longrightarrow>
+            distance_set (Graph.digraph_abs (parents bfs_state)) (t_set srcs) v =
+                 distance_set (Graph.digraph_abs (parents bfs_state)) (t_set srcs) u;
+    \<lbrakk>v \<in> t_set (current bfs_state);
+            distance_set (Graph.digraph_abs (parents bfs_state)) (t_set srcs) v = 
+              distance_set (Graph.digraph_abs (parents bfs_state)) (t_set srcs) u\<rbrakk> \<Longrightarrow>
+            u \<in> t_set (current bfs_state)\<rbrakk> \<Longrightarrow> P)
+     \<Longrightarrow> P"
+  unfolding invar_3_1'_def
+  by blast
+
+lemma invar_3_1'_intro[invar_props_intros]:
+   "\<lbrakk>\<And>u v. \<lbrakk>v \<in> t_set (current bfs_state); u \<in> t_set (current bfs_state)\<rbrakk> \<Longrightarrow>
+            distance_set (Graph.digraph_abs (parents bfs_state)) (t_set srcs) v =
+                           distance_set (Graph.digraph_abs (parents bfs_state)) (t_set srcs) u;
+     \<And>u v. \<lbrakk>v \<in> t_set (current bfs_state); distance_set (Graph.digraph_abs (parents bfs_state)) (t_set srcs) v =
+                 distance_set (Graph.digraph_abs (parents bfs_state)) (t_set srcs) u\<rbrakk> \<Longrightarrow>
+            u \<in> t_set (current bfs_state)\<rbrakk>
+    \<Longrightarrow> invar_3_1' bfs_state"
+  unfolding invar_3_1'_def
+  by blast
 
 
+definition "invar_3_2 bfs_state \<equiv> 
+  (\<forall>v\<in>t_set (current bfs_state). \<forall>u \<in> t_set (visited bfs_state).
+     distance_set (Graph.digraph_abs G) (t_set srcs) u \<le>
+       distance_set (Graph.digraph_abs G) (t_set srcs) v)"
+
+lemma invar_3_2_props[elim]: 
+  "invar_3_2 bfs_state \<Longrightarrow> 
+  (\<lbrakk>\<And>v u. \<lbrakk>v\<in>t_set (current bfs_state); u \<in> t_set (visited bfs_state)\<rbrakk> \<Longrightarrow>
+          distance_set (Graph.digraph_abs G) (t_set srcs) u \<le>
+       distance_set (Graph.digraph_abs G) (t_set srcs) v\<rbrakk> \<Longrightarrow> P)
+     \<Longrightarrow> P"
+  unfolding invar_3_2_def
+  by blast
+
+lemma invar_3_2_intro[invar_props_intros]:
+   "\<lbrakk>\<And>v u. \<lbrakk>v\<in>t_set (current bfs_state); u \<in> t_set (visited bfs_state)\<rbrakk> \<Longrightarrow>
+          distance_set (Graph.digraph_abs G) (t_set srcs) u \<le>
+       distance_set (Graph.digraph_abs G) (t_set srcs) v\<rbrakk>
+    \<Longrightarrow> invar_3_2 bfs_state"
+  unfolding invar_3_2_def
+  by blast
+
+definition "invar_3_3 bfs_state \<equiv> 
+  (\<forall>v\<in>t_set (visited bfs_state) - t_set (current bfs_state).
+     neighbourhood (Graph.digraph_abs G) v \<subseteq> t_set (visited bfs_state))"
+
+lemma invar_3_3_props[elim]: 
+  "invar_3_3 bfs_state \<Longrightarrow> 
+  (\<lbrakk>\<And>v. \<lbrakk>v \<in> t_set (visited bfs_state) - t_set (current bfs_state)\<rbrakk> \<Longrightarrow>
+          neighbourhood (Graph.digraph_abs G) v \<subseteq> t_set (visited bfs_state)\<rbrakk> \<Longrightarrow> P)
+     \<Longrightarrow> P"
+  unfolding invar_3_3_def
+  by blast
+
+lemma invar_3_3_intro[invar_props_intros]:
+   "\<lbrakk>\<And>v. \<lbrakk>v \<in> t_set (visited bfs_state) - t_set (current bfs_state)\<rbrakk> \<Longrightarrow>
+          neighbourhood (Graph.digraph_abs G) v \<subseteq> t_set (visited bfs_state)\<rbrakk>
+    \<Longrightarrow> invar_3_3 bfs_state"
+  unfolding invar_3_3_def
+  by blast
+
+\<comment> \<open>This is invar 4 on the board\<close>
+
+definition "invar_3_4 bfs_state \<equiv> 
+  (\<forall>v\<in> t_set (current bfs_state).
+     \<forall>u. distance_set (Graph.digraph_abs G) (t_set srcs) u \<le>
+           distance_set (Graph.digraph_abs G) (t_set srcs) v
+             \<longrightarrow> u \<in> t_set (visited bfs_state))"
+
+lemma invar_3_4_props[elim]: 
+  "invar_3_4 bfs_state \<Longrightarrow> 
+  (\<lbrakk>\<And>u v. \<lbrakk>v\<in> t_set (current bfs_state); distance_set (Graph.digraph_abs G) (t_set srcs) u \<le>
+           distance_set (Graph.digraph_abs G) (t_set srcs) v\<rbrakk> \<Longrightarrow>
+            u \<in> t_set (visited bfs_state)\<rbrakk> \<Longrightarrow> P)
+     \<Longrightarrow> P"
+  by(auto simp: invar_3_4_def)
+
+lemma invar_3_4_intro[invar_props_intros]:
+   "\<lbrakk>\<And>u v. \<lbrakk>v\<in> t_set (current bfs_state); distance_set (Graph.digraph_abs G) (t_set srcs) u \<le>
+           distance_set (Graph.digraph_abs G) (t_set srcs) v\<rbrakk> \<Longrightarrow>
+            u \<in> t_set (visited bfs_state)\<rbrakk>
+    \<Longrightarrow> invar_3_4 bfs_state"
+  by(auto simp add: invar_3_4_def)
+
+definition "invar_current_reachable bfs_state \<equiv> 
+  (\<forall>v\<in> t_set (visited bfs_state). distance_set (Graph.digraph_abs G) (t_set srcs) v < \<infinity>)"
+
+lemma invar_current_reachable_props[elim]: 
+  "invar_current_reachable bfs_state \<Longrightarrow> 
+  (\<lbrakk>\<And>v. \<lbrakk>v \<in> t_set (visited bfs_state)\<rbrakk> \<Longrightarrow> distance_set (Graph.digraph_abs G) (t_set srcs) v < \<infinity>\<rbrakk> \<Longrightarrow> P)
+     \<Longrightarrow> P"
+  by(auto simp: invar_current_reachable_def)
+
+lemma invar_current_reachable_intro[invar_props_intros]:
+   "\<lbrakk>\<And>v. \<lbrakk>v \<in> t_set (visited bfs_state)\<rbrakk> \<Longrightarrow> distance_set (Graph.digraph_abs G) (t_set srcs) v < \<infinity>\<rbrakk> 
+    \<Longrightarrow> invar_current_reachable bfs_state"
+  by(auto simp add: invar_current_reachable_def)
+
+lemma dist_current_plus_1:                                               
+  assumes
+    "invar_1 bfs_state" "invar_3_4 bfs_state" 
+    "v \<in> neighbourhood (Graph.digraph_abs G) v'" 
+    "v' \<in> t_set (current bfs_state)"
+    "v \<in> t_set (current (BFS_upd1 bfs_state))"
+  shows  "distance_set (Graph.digraph_abs G) (t_set srcs) v = 
+            distance_set (Graph.digraph_abs G) (t_set srcs) v' + 1" (is "?dv = ?dv' + 1")
+  proof-
+    have False if "?dv > ?dv' + 1"
+      using distance_set_neighbourhood[OF \<open>v \<in> neighbourhood (Graph.digraph_abs G) v'\<close>] that
+      by (simp add: leD)
 
 
-
-    then show ?case
-      apply(auto s imp: BFS_upd1_def)
-  next
-    case 2
-    then show ?case sorry
+    moreover have False if "?dv < ?dv' + 1"
+    proof-
+      have "?dv \<le> ?dv'"
+        using that eSuc_plus_1 ileI1
+        by force
+      moreover have "v \<notin> t_set (visited bfs_state)"
+        using assms
+        by (auto simp: BFS_upd1_def Let_def elim!: invar_1_props invar_2_props)
+      ultimately show False
+        using \<open>invar_3_4 bfs_state\<close> \<open>v' \<in> t_set (current bfs_state)\<close>
+        by auto
+    qed
+    ultimately show ?thesis
+      by force
   qed
 
-  apply(subst BFS_upd1_def)
-  apply(rule invar_props_intros)
-  apply simp
-  apply(subst expand_tree(2))
-  apply (auto elim!: call_cond_elims invar_1_props invar_2_props invar_3_props  intro!: invar_props_intros)
-  subgoal sorry
- 
-lemma invar_3_holds_4[invar_holds_intros]:
-  "\<lbrakk>BFS_ret_1_conds bfs_state; invar_3 bfs_state\<rbrakk> \<Longrightarrow> invar_3 (BFS_ret1 bfs_state)"
+
+lemma plus_lt_enat: "\<lbrakk>(a::enat) \<noteq> \<infinity>; b < c\<rbrakk> \<Longrightarrow> a + b < a + c"
+  using enat_add_left_cancel_less
+  by presburger
+
+lemma plus_one_side_lt_enat: "\<lbrakk>(a::enat) \<noteq> \<infinity>; 0 < b\<rbrakk> \<Longrightarrow> a < a + b"
+  using plus_lt_enat
+  by auto
+
+lemma invar_3_1_holds_upd1[invar_holds_intros]: 
+  "\<lbrakk>BFS_call_1_conds bfs_state; invar_1 bfs_state; invar_2 bfs_state ; invar_3_1 bfs_state;
+    invar_3_2 bfs_state; invar_3_4 bfs_state; invar_current_reachable bfs_state\<rbrakk>
+     \<Longrightarrow> invar_3_1 (BFS_upd1 bfs_state)"
+proof(intro invar_props_intros, goal_cases)
+  case assms: (1 u v)
+  obtain u' v' where uv'[intro]: "u \<in> neighbourhood (Graph.digraph_abs G) u'" "u' \<in> t_set (current bfs_state)" 
+                          "v \<in> neighbourhood (Graph.digraph_abs G) v'" "v' \<in> t_set (current bfs_state)"
+    using assms(1,2,8,9)    
+    by (auto simp: BFS_upd1_def Let_def elim!: invar_1_props)
+  moreover hence "distance_set (Graph.digraph_abs G) (t_set srcs) v' =
+                    distance_set (Graph.digraph_abs G) (t_set srcs) u'" (is "?d v' = ?d u'")
+    using \<open>invar_3_1 bfs_state\<close>
+    by auto
+  moreover have "distance_set (Graph.digraph_abs G) (t_set srcs) v = ?d v' + 1"
+    using assms
+    by (auto intro!: dist_current_plus_1)
+  moreover have "distance_set (Graph.digraph_abs G) (t_set srcs) u = ?d u' + 1"
+    using assms
+    by (auto intro!: dist_current_plus_1)
+  ultimately show ?case
+    by auto
+next
+  case (2 u v)
+  then obtain v' where uv'[intro]:
+    "v \<in> neighbourhood (Graph.digraph_abs G) v'" "v' \<in> t_set (current bfs_state)"    
+    by (auto simp: BFS_upd1_def Let_def elim!: invar_1_props invar_2_props)
+  hence "distance_set (Graph.digraph_abs G) (t_set srcs) v = 
+           distance_set (Graph.digraph_abs G) (t_set srcs) v' + 1" (is "?d v = ?d v' + _")
+    using 2
+    by(fastforce intro!: dist_current_plus_1)
+
+  show ?case
+  proof(cases "0 < ?d u")
+    case in_srcs: True
+    moreover have "?d v' < \<infinity>"
+      using \<open>?d v = ?d u\<close> \<open>invar_1 bfs_state\<close> \<open>invar_2 bfs_state\<close> \<open>v' \<in> t_set (current bfs_state)\<close>
+            \<open>invar_current_reachable bfs_state\<close>
+      by (auto elim!: invar_1_props invar_2_props invar_current_reachable_props)
+    hence "?d v < \<infinity>"
+      using \<open>?d v = ?d v' + 1\<close>
+      by (simp add: plus_eq_infty_iff_enat)
+    hence "?d u < \<infinity>"
+      using \<open>?d v = ?d u\<close>
+      by auto
+    ultimately obtain u' where "?d u' + 1 = ?d u" "u \<in> neighbourhood (Graph.digraph_abs G) u'"
+      using distance_set_parent'
+      by (metis srcs_nempty)
+    hence "?d u' = ?d v'"
+      using \<open>?d v = ?d v' + 1\<close> \<open>?d v = ?d u\<close>
+      by auto
+    hence "u' \<in> t_set (current bfs_state)"
+      using \<open>invar_3_1 bfs_state\<close>
+            \<open>v' \<in> t_set (current bfs_state)\<close>
+      by (auto elim!: invar_3_1_props)
+    moreover have "?d u' < ?d u"
+      using \<open>?d u < \<infinity>\<close> 
+      using zero_less_one not_infinity_eq 
+      by (fastforce intro!: plus_one_side_lt_enat simp: \<open>?d u' + 1 = ?d u\<close>[symmetric])
+    hence "u \<notin> t_set (visited bfs_state)"
+      using \<open>invar_3_2 bfs_state\<close> \<open>u' \<in> t_set (current bfs_state)\<close> 
+      by (auto elim!: invar_3_2_props dest: leD)
+    ultimately show ?thesis
+      using \<open>invar_1 bfs_state\<close> \<open>invar_2 bfs_state\<close> \<open>u \<in> neighbourhood (Graph.digraph_abs G) u'\<close>
+      by(fastforce simp: BFS_upd1_def Let_def elim!: invar_1_props invar_2_props)
+  next
+    case not_in_srcs: False
+    text \<open>Contradiction because if \<open>u \<in> srcs\<close> then distance srcs to a vertex in srcs is > 0. This is
+          because the distance from srcs to \<open>u\<close> is the same as that to \<open>v\<close>.\<close>
+    then show ?thesis
+      using \<open>?d v = ?d u\<close> \<open>?d v = ?d v' + 1\<close>
+      by auto
+  qed
+qed
+
+lemma invar_3_1_holds_4[invar_holds_intros]:
+  "\<lbrakk>BFS_ret_1_conds bfs_state; invar_3_3 bfs_state\<rbrakk> \<Longrightarrow> invar_3_3 (BFS_ret1 bfs_state)"
   by (auto simp: intro: invar_props_intros)
 
-lemma invar_3_holds: 
-   assumes "BFS_dom bfs_state" "invar_1 bfs_state" "invar_3 bfs_state"
-   shows "invar_3 (BFS bfs_state)"
+
+lemma invar_3_1'_holds_upd1[invar_holds_intros]: 
+  "\<lbrakk>BFS_call_1_conds bfs_state; invar_1 bfs_state; invar_2 bfs_state ; invar_3_1' bfs_state;
+    invar_3_2 bfs_state; invar_3_4 bfs_state; invar_current_reachable bfs_state\<rbrakk>
+     \<Longrightarrow> invar_3_1' (BFS_upd1 bfs_state)"
+proof(intro invar_props_intros, goal_cases)
+  case assms: (1 u v)
+  obtain u' v' where uv'[intro]: "u \<in> neighbourhood (Graph.digraph_abs (parents (BFS_upd1 bfs_state))) u'" "u' \<in> t_set (current bfs_state)" 
+                          "v \<in> neighbourhood (Graph.digraph_abs (parents (BFS_upd1 bfs_state))) v'" "v' \<in> t_set (current bfs_state)"
+    using assms(1,2,8,9)
+    apply (auto simp: BFS_upd1_def Let_def elim!: invar_1_props)
+    by (metis (no_types, lifting) case_prodI mem_Collect_eq neighbourhoodD)
+
+  moreover hence "distance_set (Graph.digraph_abs (parents bfs_state)) (t_set srcs) v' =
+                    distance_set (Graph.digraph_abs (parents bfs_state)) (t_set srcs) u'" (is "?d v' = ?d u'")
+    using \<open>invar_3_1' bfs_state\<close>
+    by auto
+  moreover have "distance_set (Graph.digraph_abs (parents (BFS_upd1 bfs_state))) (t_set srcs) v = ?d v' + 1"
+    using assms
+    by (auto intro!: dist_curr ent_plus_1)
+  oops
+
+  moreover have "distance_set (Graph.digraph_abs (parents bfs_state)) (t_set srcs) u = ?d u' + 1"
+    using assms
+    by (auto intro!: dist_current_plus_1)
+  ultimately show ?case
+    by auto
+next
+  case (2 u v)
+  then obtain v' where uv'[intro]:
+    "v \<in> neighbourhood (Graph.digraph_abs G) v'" "v' \<in> t_set (current bfs_state)"    
+    by (auto simp: BFS_upd1_def Let_def elim!: invar_1_props invar_2_props)
+  hence "distance_set (Graph.digraph_abs G) (t_set srcs) v = 
+           distance_set (Graph.digraph_abs G) (t_set srcs) v' + 1" (is "?d v = ?d v' + _")
+    using 2
+    by(fastforce intro!: dist_current_plus_1)
+
+  show ?case
+  proof(cases "0 < ?d u")
+    case in_srcs: True
+    moreover have "?d v' < \<infinity>"
+      using \<open>?d v = ?d u\<close> \<open>invar_1 bfs_state\<close> \<open>invar_2 bfs_state\<close> \<open>v' \<in> t_set (current bfs_state)\<close>
+            \<open>invar_current_reachable bfs_state\<close>
+      by (auto elim!: invar_1_props invar_2_props invar_current_reachable_props)
+    hence "?d v < \<infinity>"
+      using \<open>?d v = ?d v' + 1\<close>
+      by (simp add: plus_eq_infty_iff_enat)
+    hence "?d u < \<infinity>"
+      using \<open>?d v = ?d u\<close>
+      by auto
+    ultimately obtain u' where "?d u' + 1 = ?d u" "u \<in> neighbourhood (Graph.digraph_abs G) u'"
+      using distance_set_parent'
+      by (metis srcs_nempty)
+    hence "?d u' = ?d v'"
+      using \<open>?d v = ?d v' + 1\<close> \<open>?d v = ?d u\<close>
+      by auto
+    hence "u' \<in> t_set (current bfs_state)"
+      using \<open>invar_3_1' bfs_state\<close>
+            \<open>v' \<in> t_set (current bfs_state)\<close>
+      by (auto elim!: invar_3_1'_props)
+    moreover have "?d u' < ?d u"
+      using \<open>?d u < \<infinity>\<close> 
+      using zero_less_one not_infinity_eq 
+      by (fastforce intro!: plus_one_side_lt_enat simp: \<open>?d u' + 1 = ?d u\<close>[symmetric])
+    hence "u \<notin> t_set (visited bfs_state)"
+      using \<open>invar_3_2 bfs_state\<close> \<open>u' \<in> t_set (current bfs_state)\<close> 
+      by (auto elim!: invar_3_2_props dest: leD)
+    ultimately show ?thesis
+      using \<open>invar_1 bfs_state\<close> \<open>invar_2 bfs_state\<close> \<open>u \<in> neighbourhood (Graph.digraph_abs G) u'\<close>
+      by(fastforce simp: BFS_upd1_def Let_def elim!: invar_1_props invar_2_props)
+  next
+    case not_in_srcs: False
+    text \<open>Contradiction because if \<open>u \<in> srcs\<close> then distance srcs to a vertex in srcs is > 0. This is
+          because the distance from srcs to \<open>u\<close> is the same as that to \<open>v\<close>.\<close>
+    then show ?thesis
+      using \<open>?d v = ?d u\<close> \<open>?d v = ?d v' + 1\<close>
+      by auto
+  qed
+qed
+
+lemma invar_3_1'_holds_4[invar_holds_intros]:
+  "\<lbrakk>BFS_ret_1_conds bfs_state; invar_3_3 bfs_state\<rbrakk> \<Longrightarrow> invar_3_3 (BFS_ret1 bfs_state)"
+  by (auto simp: intro: invar_props_intros)
+
+
+
+
+lemma invar_3_2_holds_upd1[invar_holds_intros]: 
+  "\<lbrakk>BFS_call_1_conds bfs_state; invar_1 bfs_state; invar_2 bfs_state ; invar_3_1 bfs_state; 
+    invar_3_2 bfs_state; invar_3_4 bfs_state; invar_current_reachable bfs_state\<rbrakk>
+   \<Longrightarrow> invar_3_2 (BFS_upd1 bfs_state)"
+proof(intro invar_props_intros, goal_cases)                                                                          
+  case assms: (1 u v)
+  show ?case
+  proof(cases "v \<in> t_set (current (BFS_upd1 bfs_state))")
+    case v_in_current: True
+    moreover have "invar_3_1 (BFS_upd1 bfs_state)"
+      using assms
+      by (auto intro: invar_holds_intros)
+    ultimately show ?thesis
+      using \<open>u \<in> t_set (current (BFS_upd1 bfs_state))\<close>
+      by fastforce
+  next                     
+    case v_not_in_current: False
+    hence "v \<in> t_set (visited bfs_state)"
+      using assms(1,2,9)
+      by (fastforce simp: BFS_upd1_def Let_def elim!: invar_1_props)
+    moreover obtain u' where uv'[intro]: "u \<in> neighbourhood (Graph.digraph_abs G) u'" "u' \<in> t_set (current bfs_state)" 
+      using assms(1,2,8,9)    
+      by (auto simp: BFS_upd1_def Let_def elim!: invar_1_props)
+    ultimately have "distance_set (Graph.digraph_abs G) (t_set srcs) v \<le>
+                       distance_set (Graph.digraph_abs G) (t_set srcs) u'"
+      using \<open>invar_3_2 bfs_state\<close>
+      by (auto elim!: invar_3_2_props)
+    moreover have "distance_set (Graph.digraph_abs G) (t_set srcs) u = 
+           distance_set (Graph.digraph_abs G) (t_set srcs) u' + 1" (is "?d u = ?d u' + _")
+      using assms
+      by(fastforce intro!: dist_current_plus_1)
+    ultimately show ?thesis
+      by (metis le_iff_add order.trans)
+  qed
+qed
+
+lemma invar_3_2_holds_4[invar_holds_intros]:
+  "\<lbrakk>BFS_ret_1_conds bfs_state; invar_3_3 bfs_state\<rbrakk> \<Longrightarrow> invar_3_3 (BFS_ret1 bfs_state)"
+  by (auto simp: intro: invar_props_intros)
+
+lemma invar_3_3_holds_upd1[invar_holds_intros]: 
+  "\<lbrakk>BFS_call_1_conds bfs_state; invar_1 bfs_state; invar_2 bfs_state; invar_3_3 bfs_state\<rbrakk> \<Longrightarrow> invar_3_3 (BFS_upd1 bfs_state)"
+  apply(auto elim!: call_cond_elims invar_1_props invar_2_props invar_3_3_props intro!: invar_props_intros simp: BFS_upd1_def Let_def)
+  by (metis in_mono)+
+
+lemma invar_3_3_holds_4[invar_holds_intros]:
+  "\<lbrakk>BFS_ret_1_conds bfs_state; invar_3_3 bfs_state\<rbrakk> \<Longrightarrow> invar_3_3 (BFS_ret1 bfs_state)"
+  by (auto simp: intro: invar_props_intros)
+
+lemma invar_3_4_holds_upd1[invar_holds_intros]: 
+  "\<lbrakk>BFS_call_1_conds bfs_state; invar_1 bfs_state; invar_2 bfs_state;
+    invar_3_1 bfs_state; invar_3_2 bfs_state; invar_3_3 bfs_state; invar_3_4 bfs_state;
+    invar_current_reachable bfs_state\<rbrakk> \<Longrightarrow> 
+    invar_3_4 (BFS_upd1 bfs_state)"
+proof(intro invar_props_intros, goal_cases)                                                                                                    
+  case assms: (1 u v)
+  then obtain v' where v'[intro]:
+                          "v \<in> neighbourhood (Graph.digraph_abs G) v'" "v' \<in> t_set (current bfs_state)"    
+    by (force simp: BFS_upd1_def Let_def)
+  have "distance_set (Graph.digraph_abs G) (t_set srcs) v = distance_set (Graph.digraph_abs G) (t_set srcs) v' + 1" (is "?dv = ?dv' + 1")
+    using assms
+    by (auto intro!: dist_current_plus_1)
+  moreover have "u \<in> t_set (visited (BFS_upd1 bfs_state))"
+    if "distance_set (Graph.digraph_abs G) (t_set srcs) u \<le> ?dv'" (is "?du \<le> ?dv'")
+      using that \<open>invar_1 bfs_state\<close> \<open>invar_3_4 bfs_state\<close> 
+      by (fastforce simp: BFS_upd1_def Let_def)
+  moreover have "u \<in> t_set (visited (BFS_upd1 bfs_state))"
+    if "distance_set (Graph.digraph_abs G) (t_set srcs) u = ?dv"
+  proof-
+    have "invar_3_1 (BFS_upd1 bfs_state)"
+      by (auto intro: assms invar_holds_intros)
+    hence "u \<in> t_set (current (BFS_upd1 bfs_state))"
+      using that \<open>invar_3_1 bfs_state\<close> \<open>v \<in> t_set (current (BFS_upd1 bfs_state))\<close>
+      by (auto elim!: invar_3_1_props) 
+    then obtain u' where u'[intro]:
+                         "u \<in> neighbourhood (Graph.digraph_abs G) u'"
+                         "u' \<in> t_set (current bfs_state)"
+       using assms
+      by (auto simp: BFS_upd1_def Let_def elim!: invar_1_props)
+    hence "distance_set (Graph.digraph_abs G) (t_set srcs) u = distance_set (Graph.digraph_abs G) (t_set srcs) u' + 1"
+      using assms(2) assms(7) \<open>u \<in> t_set (current (BFS_upd1 bfs_state))\<close> dist_current_plus_1
+      by blast
+    hence "distance_set (Graph.digraph_abs G) (t_set srcs) u' \<le> distance_set (Graph.digraph_abs G) (t_set srcs) v'" (is "?du' \<le> _")
+      using that \<open>?dv = ?dv' +1\<close>
+      by auto
+    hence "u' \<in> t_set (visited bfs_state)"
+      using \<open>invar_3_4 bfs_state\<close>
+      by auto
+    hence "u' \<in> t_set (current bfs_state) \<or> u' \<in> t_set (visited bfs_state) - t_set (current bfs_state)"
+      by auto
+    thus ?thesis
+    proof(elim disjE, goal_cases)
+      case 1
+      thus ?case
+        using \<open>u \<in> neighbourhood (Graph.digraph_abs G) u'\<close> \<open>invar_1 bfs_state\<close> \<open>invar_2 bfs_state\<close>
+        by (fastforce simp: BFS_upd1_def Let_def elim!: invar_1_props invar_2_props)
+    next
+      case 2
+      then show ?case
+        using \<open>u \<in> neighbourhood (Graph.digraph_abs G) u'\<close> \<open>invar_1 bfs_state\<close>
+              \<open>invar_3_3 bfs_state\<close>
+        by (fastforce simp: BFS_upd1_def Let_def)
+    qed
+  qed
+  ultimately show ?case
+    using \<open>?du \<le> ?dv\<close> ileI1 linorder_not_less plus_1_eSuc(2)
+    by fastforce
+qed
+
+lemma invar_3_4_holds_4[invar_holds_intros]:
+  "\<lbrakk>BFS_ret_1_conds bfs_state; invar_3_4 bfs_state\<rbrakk> \<Longrightarrow> invar_3_4 (BFS_ret1 bfs_state)"
+  by (auto simp: intro: invar_props_intros)
+
+
+definition "invar_dist bfs_state \<equiv> 
+  (\<forall>v \<in> dVs (Graph.digraph_abs G).
+     (\<comment>\<open>v \<in> t_set (visited bfs_state) \<longrightarrow> \<close>distance_set (Graph.digraph_abs G) (t_set srcs) v =
+         distance_set (Graph.digraph_abs (parents bfs_state)) (t_set srcs) v) \<and>
+       (\<comment>\<open>v \<notin> t_set (visited bfs_state) \<longrightarrow> \<close>(\<exists>u\<in>t_set (current bfs_state). distance_set (Graph.digraph_abs G) (t_set srcs) v =
+                                        distance_set (Graph.digraph_abs (parents bfs_state)) (t_set srcs) u +
+                                         distance_set (Graph.digraph_abs G) (t_set (current bfs_state)) v)))"
+                                      
+lemma invar_dist_props[elim]: 
+  "invar_dist bfs_state \<Longrightarrow> v \<in> dVs (Graph.digraph_abs G) \<Longrightarrow> 
+   \<lbrakk>
+     \<lbrakk>\<comment>\<open>v \<in> t_set (visited bfs_state); \<close>distance_set (Graph.digraph_abs G) (t_set srcs) v =
+         distance_set (Graph.digraph_abs (parents bfs_state)) (t_set srcs) v\<rbrakk> \<Longrightarrow> P;
+     \<And>u.\<lbrakk>\<comment>\<open>v \<notin> t_set (visited bfs_state); \<close>u\<in>t_set (current bfs_state);
+            distance_set (Graph.digraph_abs G) (t_set srcs) v =  
+              distance_set (Graph.digraph_abs (parents bfs_state)) (t_set srcs) u +
+                distance_set (Graph.digraph_abs G) (t_set (current bfs_state)) v\<rbrakk> \<Longrightarrow> P
+   \<rbrakk>                                                                                              
+   \<Longrightarrow> P"
+  unfolding invar_dist_def
+  by auto
+
+lemma invar_dist_intro[invar_props_intros]:
+   "\<lbrakk>\<And>v. \<lbrakk>v \<in> dVs (Graph.digraph_abs G)\<comment>\<open>; v \<in> t_set (visited bfs_state)\<close>\<rbrakk> \<Longrightarrow> 
+           (distance_set (Graph.digraph_abs G) (t_set srcs) v =
+             distance_set (Graph.digraph_abs (parents bfs_state)) (t_set srcs) v);
+     \<And>v. \<lbrakk>v \<in> dVs (Graph.digraph_abs G)\<comment>\<open>; v \<notin> t_set (visited bfs_state)\<close>\<rbrakk> \<Longrightarrow>
+            (\<exists>u\<in>t_set (current bfs_state).
+                    distance_set (Graph.digraph_abs G) (t_set srcs) v =
+                      distance_set (Graph.digraph_abs (parents bfs_state)) (t_set srcs) u +
+                        distance_set (Graph.digraph_abs G) (t_set (current bfs_state)) v)\<rbrakk>
+        
+    \<Longrightarrow> invar_dist bfs_state"
+  unfolding invar_dist_def
+  by auto
+
+definition "invar_dist' bfs_state \<equiv> 
+  (\<forall>v \<in> dVs (Graph.digraph_abs G).
+     (v \<in> t_set (visited bfs_state) \<longrightarrow> distance_set (Graph.digraph_abs G) (t_set srcs) v =
+         distance_set (Graph.digraph_abs (parents bfs_state)) (t_set srcs) v))"
+                                      
+lemma invar_dist'_props[elim]: 
+  "invar_dist' bfs_state \<Longrightarrow> v \<in> dVs (Graph.digraph_abs G) \<Longrightarrow> 
+   \<lbrakk>
+     \<lbrakk>v \<in> t_set (visited bfs_state) \<Longrightarrow> distance_set (Graph.digraph_abs G) (t_set srcs) v =
+         distance_set (Graph.digraph_abs (parents bfs_state)) (t_set srcs) v\<rbrakk> \<Longrightarrow> P
+   \<rbrakk>
+   \<Longrightarrow> P"
+  unfolding invar_dist'_def
+  by auto
+
+lemma invar_dist'_intro[invar_props_intros]:
+   "\<lbrakk>\<And>v. \<lbrakk>v \<in> dVs (Graph.digraph_abs G); v \<in> t_set (visited bfs_state)\<rbrakk> \<Longrightarrow> 
+           (distance_set (Graph.digraph_abs G) (t_set srcs) v =
+             distance_set (Graph.digraph_abs (parents bfs_state)) (t_set srcs) v)\<rbrakk>
+        
+    \<Longrightarrow> invar_dist' bfs_state"
+  unfolding invar_dist'_def
+  by auto
+
+lemma distance_next_frontier: 
+  "\<lbrakk>invar_1 BFS_state; invar_2 BFS_state; 
+        v \<in> t_set (next_frontier (current BFS_state) (visited BFS_state))\<rbrakk>
+         \<Longrightarrow> distance_set (Graph.digraph_abs G) (t_set (current BFS_state)) v = 1"
+proof(goal_cases)
+  case assms: 1
+  then obtain u where "u \<in> t_set (current BFS_state)" "v \<in> neighbourhood (Graph.digraph_abs G) u"
+    by force
+  hence "v \<notin> t_set (current BFS_state)"
+    using assms
+    by force
+  hence "u \<noteq> v" if "u \<in> t_set (current BFS_state)" for u                                                                         
+    using that 
+    by auto
+  hence "distance (Graph.digraph_abs G) u v \<noteq> 0"  if "u \<in> t_set (current BFS_state)" for u
+    using distance_0 that
+    by metis
+  hence "distance (Graph.digraph_abs G) u v = 1"
+    using distance_neighbourhood \<open>u \<in> t_set (current BFS_state)\<close>
+          \<open>v \<in> neighbourhood (Graph.digraph_abs G) u\<close> iless_eSuc0 one_eSuc
+    by fastforce
+  thus ?thesis
+    by (metis \<open>u \<in> t_set (current BFS_state)\<close> \<open>v \<notin> t_set (current BFS_state)\<close> dist_not_inf'
+              dist_set_mem distance_0 iless_eSuc0 infinity_ileE one_eSuc one_enat_def
+              order_le_imp_less_or_eq)
+qed
+
+lemma dist_tree_visited:
+  "\<lbrakk>invar_1 bfs_state; invar_2 bfs_state; invar_dist bfs_state; v \<in> t_set (visited bfs_state)\<rbrakk> \<Longrightarrow> 
+     distance_set (Graph.digraph_abs G) (t_set srcs) v = 
+       distance_set (Graph.digraph_abs (parents bfs_state)) (t_set srcs) v" (is "\<lbrakk>_; _; _; _\<rbrakk> \<Longrightarrow> ?dSrcsG v = ?dSrcsT v")
+proof(goal_cases)
+  case 1
+  have "?dSrcsG v \<le>  ?dSrcsT v"
+  proof(rule ccontr, goal_cases)
+    case 1
+    hence "?dSrcsG v \<noteq>  ?dSrcsT v"
+      by auto
+    then obtain u where "u \<in> t_set (current bfs_state)"
+                        "?dSrcsG v =  ?dSrcsT u +
+                              distance_set (Graph.digraph_abs G) (t_set (current bfs_state)) v"
+      using  \<open>invar_dist bfs_state\<close> \<open>v \<in> t_set (visited bfs_state)\<close> \<open>invar_2 bfs_state\<close>
+      by (force elim!: invar_dist_props dest: dVs_subset)
+
+    then show ?case sorry
+  qed
+  oops
+
+definition "invar_goes_through_current bfs_state \<equiv> 
+         (\<forall>u\<in>t_set (visited bfs_state). 
+            \<forall>v. v \<notin> t_set (visited bfs_state) \<longrightarrow>
+              (\<forall>p. Vwalk.vwalk_bet (Graph.digraph_abs G) u p v \<longrightarrow> 
+                     set p \<inter> t_set (current bfs_state) \<noteq> {}))"
+
+lemma invar_goes_through_current_props[elim]: 
+  "invar_goes_through_current  bfs_state \<Longrightarrow> 
+   \<lbrakk>\<lbrakk>\<And>u v p. \<lbrakk>u \<in>t_set (visited bfs_state); v \<notin> t_set (visited bfs_state); 
+              Vwalk.vwalk_bet (Graph.digraph_abs G) u p v\<rbrakk>
+      \<Longrightarrow> set p \<inter> t_set (current bfs_state) \<noteq> {}\<rbrakk>
+     \<Longrightarrow> P\<rbrakk>
+   \<Longrightarrow> P"
+  unfolding invar_goes_through_current_def
+  by auto
+
+lemma invar_goes_through_current_intro[invar_props_intros]:
+  "\<lbrakk>\<And>u v p. \<lbrakk>u \<in>t_set (visited bfs_state); v \<notin> t_set (visited bfs_state); 
+              Vwalk.vwalk_bet (Graph.digraph_abs G) u p v\<rbrakk>
+      \<Longrightarrow> set p \<inter> t_set (current bfs_state) \<noteq> {}\<rbrakk>
+    \<Longrightarrow> invar_goes_through_current bfs_state"
+  unfolding invar_goes_through_current_def
+  by auto
+end text \<open>@{term BFS}\<close>
+
+lemma list_2_preds_aux:
+  "\<lbrakk>x' \<in> set xs; P1 x'; \<And>xs1 x xs2. \<lbrakk>xs = xs1 @ [x] @ xs2; P1 x\<rbrakk> \<Longrightarrow>
+      \<exists>ys1 y ys2. x # xs2 = ys1 @ [y] @ ys2 \<and> P2 y\<rbrakk> \<Longrightarrow> 
+     \<exists> xs1 x xs2. xs = xs1 @ [x] @ xs2 \<and> P2 x \<and> (\<forall>y\<in>set xs2. \<not> P1 y)"
+proof(goal_cases)
+  case assms: 1
+
+
+  define property 
+       where "property xs \<equiv>
+                (\<forall>xs2 xs1 x. (xs = xs1 @ [x] @ xs2 \<and> P1 x) \<longrightarrow>
+                   (\<exists>ys1 y ys2. x#xs2 = ys1 @ [y] @ ys2 \<and> P2 y))"
+       for xs
+
+  have propE: "\<lbrakk>property xs;
+               (\<And>xs1 x xs2. \<lbrakk>xs = xs1 @ [x] @ xs2; P1 x\<rbrakk> \<Longrightarrow>
+                  \<exists>ys1 y ys2. x#xs2 = ys1 @ [y] @ ys2 \<and> P2 y) \<Longrightarrow> P\<rbrakk>
+              \<Longrightarrow> P" for xs P
+    by(auto simp add: property_def)
+
+  have property_append: "property (xs @ ys) \<Longrightarrow> property ys" for xs ys
+    by(auto simp: property_def)
+
+  have "property xs"
+    using assms(3)
+    by (force simp: property_def)
+
+
+
+  thus  ?thesis
+    using assms(1,2)
+  proof(induction xs arbitrary: x')
+    case Nil
+    then show ?case 
+      by auto
+  next
+    case (Cons a xs)
+    hence "property xs" 
+      by(auto intro: property_append[where xs = "[a]"])
+
+    show ?case
+    proof(cases "x' = a")
+      case x_eq_a: True
+
+      then obtain ys1 y ys2 where "x'#xs = ys1 @ [y] @ ys2" "P2 y"
+        using \<open>property (a # xs)\<close> \<open>P1 x'\<close>
+        by (auto 10 10 elim!: propE)
+
+      show ?thesis
+      proof(cases "ys1 = []")
+        case ys1_empty: True
+        hence "xs = ys2"
+          using \<open>x'#xs = ys1 @ [y] @ ys2\<close>
+          by auto
+        then show ?thesis
+        proof(cases "\<exists>x\<in>set ys2. P1 x")
+          case x_in_ys2: True
+          then obtain x where "x \<in> set ys2" "P1 x"
+            by auto
+          hence "\<exists>xs1 x xs2. xs = xs1 @ [x] @ xs2 \<and> P2 x \<and> (\<forall>y\<in>set xs2. \<not> P1 y)"
+            using \<open>property xs\<close> \<open>xs = ys2\<close> \<open>P2 y\<close>
+            apply(intro Cons(1))
+            by auto
+          then obtain xs1 x xs2 where "(a # xs) = (a #xs1) @ [x] @ xs2 \<and> P2 x \<and> (\<forall>y\<in>set xs2. \<not> P1 y)"
+            by auto
+          then show ?thesis
+            by metis
+        next
+          case x_notin_ys2: False
+          hence "a # xs = a#ys2 \<and> P2 y \<and> (\<forall>y\<in>set ys2. \<not> P1 y)"
+            using \<open>xs = ys2\<close> \<open>P2 y\<close>
+            by auto
+          then show ?thesis
+            using \<open>x' # xs = ys1 @ [y] @ ys2\<close> x_eq_a
+            by blast
+        qed
+      next
+        case ys2_nempty: False
+        then obtain ys1' where "xs = ys1' @ [y] @ ys2"
+          using \<open>x'#xs = ys1 @ [y] @ ys2\<close>
+          by (auto simp: neq_Nil_conv)
+        show ?thesis
+        proof(cases "\<exists>x\<in>set ys2. P1 x")
+          case x_in_ys2: True
+          then obtain x where "x \<in> set ys2" "P1 x"
+            by auto
+          hence "\<exists>xs1 x xs2. xs = xs1 @ [x] @ xs2 \<and> P2 x \<and> (\<forall>y\<in>set xs2. \<not> P1 y)"
+            using \<open>property xs\<close> \<open>xs = ys1' @ [y] @ ys2\<close> \<open>P2 y\<close>
+            apply(intro Cons(1))
+            by auto
+          then obtain xs1 x xs2 where "(a # xs) = (a #xs1) @ [x] @ xs2 \<and> P2 x \<and> (\<forall>y\<in>set xs2. \<not> P1 y)"
+            by auto
+          then show ?thesis
+            by metis
+        next
+          case x_notin_ys2: False
+          hence "a # xs = (a# ys1') @ [y] @ ys2 \<and> P2 y \<and> (\<forall>y\<in>set ys2. \<not> P1 y)"
+            using \<open>xs = ys1' @ [y] @ ys2\<close> \<open>P2 y\<close>
+            by auto
+          then show ?thesis
+            by metis
+        qed
+      qed
+    next
+      case x_neq_a: False
+      hence "x' \<in> set xs"
+        using Cons
+        by auto
+      then obtain xs1 x xs2 where "xs = xs1 @ [x] @ xs2" "P2 x" "(\<forall>y\<in>set xs2. \<not> P1 y)"
+        using Cons \<open>property xs\<close>
+        by blast
+      hence "a # xs = (a # xs1) @ [x] @ xs2 \<and> P2 x \<and> (\<forall>y\<in>set xs2. \<not> P1 y)"
+        by auto
+      thus ?thesis
+        by metis
+    qed
+  qed
+
+
+qed
+
+lemma list_2_preds:
+  "\<lbrakk> x\<in>set xs; P1 x; \<And>xs1 x xs2. \<lbrakk>xs = xs1 @ [x] @ xs2; P1 x\<rbrakk> \<Longrightarrow> \<exists>ys1 y ys2. x#xs2 = ys1 @ [y] @ ys2 \<and> P2 y\<rbrakk> \<Longrightarrow> 
+     \<exists> xs1 x xs2. xs = xs1 @ [x] @ xs2 \<and> P2 x \<and> (\<forall>y\<in>set xs2. \<not> P1 y \<and> \<not> P2 y)"
+proof(goal_cases)
+  case assms: 1
+  hence "\<exists>xs1 x xs2. xs = xs1 @ [x] @ xs2 \<and> P2 x \<and> (\<forall>y\<in>set xs2. \<not> P1 y)"
+    by (fastforce intro!: list_2_preds_aux)
+  then obtain xs1 x xs2 where "xs = xs1 @ [x] @ xs2" "P2 x" "(\<forall>y\<in>set xs2. \<not> P1 y)"
+    by auto
+  hence "\<exists>ys1 y ys2. x # xs2 = ys1 @ [y] @ ys2 \<and> P2 y \<and> (\<forall>z\<in>set ys2. \<not> P2 z)"
+    by (auto intro!: split_list_last_prop)
+  then obtain ys1 y ys2 where "x # xs2 = ys1 @ [y] @ ys2" "P2 y" "(\<forall>z\<in>set ys2. \<not> P2 z)"
+    by auto
+  hence "(\<forall>z\<in>set ys2. \<not>P1 z \<and> \<not> P2 z)"
+    using \<open>(\<forall>y\<in>set xs2. \<not> P1 y)\<close> \<open>P2 x\<close>
+    by (metis Un_iff insert_iff list.simps(15) set_append)
+  moreover have "xs = (xs1 @ ys1) @ [y] @ ys2"
+    using \<open>xs = xs1 @ [x] @ xs2\<close> \<open>x # xs2 = ys1 @ [y] @ ys2\<close>
+    by auto
+  ultimately show ?case
+    using \<open>P2 y\<close>
+    by fastforce
+qed
+
+lemma list_inter_mem_iff: "set xs \<inter> s \<noteq> {} \<longleftrightarrow> (\<exists>xs1 x xs2. xs = xs1 @ [x] @ xs2 \<and> x \<in> s)"
+  by (metis append.left_neutral append_Cons disjoint_iff in_set_conv_decomp)
+
+context BFS 
+begin
+
+
+thm list_2_preds[where ?P2.0 = "(\<lambda>x. x \<in> t_set (current bfs_state))",
+              simplified list_inter_mem_iff[symmetric]]
+
+
+lemma invar_goes_through_active_holds_upd1[invar_holds_intros]: 
+  "\<lbrakk>BFS_call_1_conds bfs_state; invar_1 bfs_state; invar_2 bfs_state; 
+    invar_goes_through_current bfs_state\<rbrakk> 
+    \<Longrightarrow> invar_goes_through_current (BFS_upd1 bfs_state)"
+proof(intro invar_props_intros, goal_cases)
+  case (1 u v p)
+  hence "v \<notin> t_set (visited bfs_state)"
+    by (auto simp: Let_def BFS_upd1_def elim!: invar_1_props invar_2_props)
+  show ?case
+  proof(cases "u \<in> t_set (visited bfs_state)")
+    case u_in_visited: True
+      have "Vwalk.vwalk_bet (Graph.digraph_abs G) u p v" "set p \<inter> t_set (current bfs_state) \<noteq> {}"
+        using \<open>invar_goes_through_current bfs_state\<close> \<open>v \<notin> t_set (visited bfs_state)\<close>
+          \<open>vwalk_bet (Graph.digraph_abs G) u p v\<close> u_in_visited
+        by (auto elim!: invar_goes_through_current_props)
+      moreover have "u \<in> set p"
+        using \<open>Vwalk.vwalk_bet (Graph.digraph_abs G) u p v\<close>
+        by(auto intro: hd_of_vwalk_bet'')
+      ultimately have "\<exists> p1 x p2. p = p1 @ [x] @ p2 \<and>
+                          x \<in> t_set (current bfs_state) \<and> 
+                          (\<forall>y\<in>set p2. y \<notin> (t_set (visited bfs_state)) \<and>
+                                      y \<notin> (t_set (current bfs_state)))"
+        using \<open>invar_goes_through_current bfs_state\<close> u_in_visited \<open>v \<notin> t_set (visited bfs_state)\<close>
+          \<open>invar_1 bfs_state\<close> \<open>invar_2 bfs_state\<close>
+        by (intro list_2_preds[where ?P2.0 = "(\<lambda>x. x \<in> t_set (current bfs_state))",
+              simplified list_inter_mem_iff[symmetric]])
+        (force elim!: invar_goes_through_current_props dest!:split_vwalk)+
+
+
+    then obtain p1 x p2 where "p = p1 @ x # p2" and
+      "x \<in> t_set (current bfs_state)" and
+      unvisited:
+      "(\<And>y. y\<in>set p2 \<Longrightarrow> y \<notin> t_set (visited bfs_state))"
+      by auto
+    moreover have "last p = v"
+      using \<open>vwalk_bet (Graph.digraph_abs G) u p v\<close>
+      by auto
+    ultimately have "v \<in> set p2"
+      using \<open>v \<notin> t_set (visited bfs_state)\<close> \<open>invar_1 bfs_state\<close> \<open>invar_2 bfs_state\<close>
+      by force
+    then obtain v' p2' where "p2 = v' # p2'"
+      by (cases p2) auto
+    hence "v' \<in> neighbourhood (Graph.digraph_abs G) x"
+      using \<open>p = p1 @ x # p2\<close> \<open>Vwalk.vwalk_bet (Graph.digraph_abs G) u p v\<close>
+        split_vwalk
+      by fastforce
+    moreover have "v' \<in> set p2"
+      using \<open>p2 = v' # p2'\<close>
+      by auto
+    ultimately have "v' \<in> t_set (current (BFS_upd1 bfs_state))"
+      using \<open>invar_1 bfs_state\<close> \<open>invar_2 bfs_state\<close> \<open>x \<in> t_set (current bfs_state)\<close> 
+      by(fastforce simp: BFS_upd1_def Let_def elim!: invar_1_props invar_2_props dest!: unvisited)
+    then show ?thesis
+      by(auto intro!: invar_goes_through_current_intro simp: \<open>p = p1 @ x # p2\<close> \<open>p2 = v' # p2'\<close>) 
+next
+  case u_not_in_visited: False
+  hence "u \<in> t_set (current (BFS_upd1 bfs_state))"
+    using \<open>invar_1 bfs_state\<close>
+      \<open>u \<in> t_set (visited (BFS_upd1 bfs_state))\<close>
+    by (auto simp: BFS_upd1_def Let_def)
+  moreover have "u \<in> set p"
+    using \<open>Vwalk.vwalk_bet (Graph.digraph_abs G) u p v\<close>
+    by (auto intro: hd_of_vwalk_bet'')
+  ultimately show ?thesis
+    by(auto intro!: invar_goes_through_current_intro)
+qed
+qed
+
+lemma invar_dist_holds_upd1[invar_holds_intros]: 
+  "\<lbrakk>BFS_call_1_conds bfs_state; invar_1 bfs_state; invar_2 bfs_state; invar_3_1 bfs_state;
+    invar_3_2 bfs_state; invar_dist bfs_state\<rbrakk> 
+    \<Longrightarrow> invar_dist (BFS_upd1 bfs_state)"
+proof(intro invar_props_intros, goal_cases)
+  define bfs_state' where "bfs_state' \<equiv> BFS_upd1 bfs_state"
+  let ?dSrcsG = "distance_set (Graph.digraph_abs G) (t_set srcs)"
+  let ?dSrcsT = "distance_set (Graph.digraph_abs (parents bfs_state)) (t_set srcs)"
+  let ?dSrcsT' = "distance_set (Graph.digraph_abs (parents bfs_state')) (t_set srcs)"
+  let ?dCurrG = "distance_set (Graph.digraph_abs G)  (t_set (current bfs_state))"
+  case (1 v)
+  then show ?case
+  proof(cases "distance_set (Graph.digraph_abs G) (t_set srcs) v = \<infinity>")
+    case infinite: True
+    moreover have "?dSrcsG v \<le> ?dSrcsT' v"
+      using \<open>invar_1 bfs_state\<close> \<open>invar_2 bfs_state\<close>
+      by(fastforce simp: bfs_state'_def BFS_upd1_def Let_def intro: distance_set_subset)    
+    ultimately show ?thesis
+      by (simp add: bfs_state'_def)
+  next
+    case finite: False
+    show ?thesis
+    proof(cases "v \<in> dVs (Graph.digraph_abs (parents bfs_state))")
+      case v_in_tree: True
+      have "?dSrcsT v = ?dSrcsG v"
+      proof(rule ccontr, goal_cases)
+        case 1
+        moreover have \<open>Graph.digraph_abs (parents bfs_state) \<subseteq> Graph.digraph_abs G\<close>
+          using \<open>invar_2 bfs_state\<close>
+          by auto
+        ultimately have "?dSrcsG v < ?dSrcsT v"
+          text \<open>because the tree is a subset of the Graph, which invar?\<close>
+          by (simp add: distance_set_subset order_less_le)
+        then obtain p where p: 
+          "p\<in>t_set (current bfs_state)"
+          "?dSrcsG v = ?dSrcsT p + ?dCurrG v"
+          using \<open>invar_dist bfs_state\<close> v_in_tree \<open>v \<in> dVs (Graph.digraph_abs G)\<close>
+          by auto
+        hence "?dSrcsT p + ?dCurrG v < ?dSrcsT v"
+          using \<open>?dSrcsG v < ?dSrcsT v\<close>
+          by simp
+        hence "?dSrcsT p < ?dSrcsT v"
+          by (meson le_iff_add order_le_less_trans)
+        moreover have "?dSrcsT p = ?dSrcsG p "
+          using \<open>p \<in> t_set (current bfs_state)\<close> \<open>invar_dist bfs_state\<close> \<open>invar_2 bfs_state\<close>
+          by (metis "1" dist_set_inf invar_dist_def local.finite)
+        moreover have "?dSrcsT v = ?dSrcsG v"
+          using v_in_tree \<open>invar_dist bfs_state\<close> \<open>invar_2 bfs_state\<close> \<open>v\<in> dVs (Graph.digraph_abs G)\<close>
+          by (metis invar_dist_def)
+        ultimately have "?dSrcsG p < ?dSrcsG v"
+          by auto
+        then show ?case
+          using \<open>invar_2 bfs_state\<close> \<open>invar_3_1 bfs_state\<close> \<open>invar_3_2 bfs_state\<close> v_in_tree
+                \<open>p \<in> t_set (current bfs_state)\<close>
+          by fastforce
+      qed
+      moreover have "?dSrcsT v = ?dSrcsT' v"
+      proof-
+        have "?dSrcsT' v \<le> ?dSrcsT v"
+          using \<open>invar_1 bfs_state\<close>
+          by(fastforce simp: bfs_state'_def BFS_upd1_def Let_def intro: distance_set_subset)
+
+        moreover have "?dSrcsG v \<le> ?dSrcsT' v"
+          using \<open>invar_1 bfs_state\<close> \<open>invar_2 bfs_state\<close>
+          by(fastforce simp: bfs_state'_def BFS_upd1_def Let_def intro: distance_set_subset)
+
+        ultimately show ?thesis
+          using \<open>?dSrcsT v = ?dSrcsG v\<close>
+          by auto
+      qed
+      ultimately show ?thesis
+        by (auto simp: bfs_state'_def)
+    next
+      case v_not_in_tree: False
+      hence "?dSrcsT v = \<infinity>"
+        by(auto intro: dist_set_inf)
+      hence "?dSrcsG v \<noteq> ?dSrcsT v"
+        using finite
+        by auto
+      then obtain u where 
+               "u\<in>t_set (current bfs_state)"
+               "?dSrcsG v = ?dSrcsT u + ?dCurrG v"
+        using \<open>invar_dist bfs_state\<close> \<open>v \<in> dVs (Graph.digraph_abs G)\<close>
+        by auto
+      have "?dCurrG v \<noteq> \<infinity>"
+        using finite \<open>?dSrcsG v = ?dSrcsT u + ?dCurrG v\<close>
+        by (simp add: plus_eq_infty_iff_enat)
+      then obtain w where "w \<in> t_set (current bfs_state)" "Pair_Graph.reachable (Graph.digraph_abs G) w v"
+                     "distance (Graph.digraph_abs G) w v = ?dCurrG v"
+        by (meson dist_not_inf')
+      find_theorems distance_set "{}"                        
+      obtain p where "vwalk_bet (Graph.digraph_abs G) w (w#p) v"
+                     "length p = distance (Graph.digraph_abs G) w v"
+                     "set p \<inter> (t_set (current bfs_state)) = {}"
+         using dist_not_inf''[OF \<open>?dCurrG v \<noteq> \<infinity>\<close> 
+                                 \<open>w \<in> t_set (current bfs_state)\<close>
+                                 \<open>distance (Graph.digraph_abs G) w v = ?dCurrG v\<close>]
+         by auto
+      hence "shortest_path (Graph.digraph_abs G) w (w#p) v"
+        by (simp add: shortest_path_def)
+      show ?thesis
+      proof(cases "distance (Graph.digraph_abs G) w v = 0")
+        case dist_w_v_0: True
+        then show ?thesis sorry
+      next
+        case dist_w_v_not_0: False
+        then obtain i where \<open>eSuc i = distance (Graph.digraph_abs G) w v\<close> 
+          using \<open>length p = distance (Graph.digraph_abs G) w v\<close>
+          by(cases p) (fastforce simp: enat_0)+
+        then obtain x p' where "p = x # p'"
+          using \<open>length p = distance (Graph.digraph_abs G) w v\<close> \<open>?dCurrG v \<noteq> \<infinity>\<close>
+                \<open>distance (Graph.digraph_abs G) w v = ?dCurrG v\<close>
+          by (cases p) (auto simp: neq_Nil_conv enat_0)
+
+        define current' where "current' \<equiv> (t_set (current bfs_state)) \<union>
+                                  (t_set (next_frontier (current bfs_state) (visited bfs_state)))"
+
+        note \<open>distance (Graph.digraph_abs G) w v = ?dCurrG v\<close>
+             \<open>w \<in> t_set (current bfs_state)\<close>
+             \<open>invar_1 bfs_state\<close> \<open>invar_2 bfs_state\<close>
+        moreover have "shortest_path (Graph.digraph_abs G) w (w#x#p') v"
+          using \<open>shortest_path (Graph.digraph_abs G) w (w#p) v\<close> \<open>p = x # p'\<close>
+          by auto
+
+        find_theorems shortest_path vwalk_bet
+
+        moreover hence "x \<in> neighbourhood (Graph.digraph_abs G) w"
+          by(auto dest!: shortest_path_vwalk)
+
+
+
+        ultimately have "distance_set (Graph.digraph_abs G) current' v =
+                           distance_set (Graph.digraph_abs G) (t_set (current bfs_state)) v -
+                             distance (Graph.digraph_abs G) w x"
+          apply (subst current'_def)
+          apply (rule shortest_path_dist_set_union[where ?p1.0 = "[w]"])
+          apply auto[1]
+          apply auto[1]          
+          apply auto[1]
+          apply (auto elim!: invar_1_props invar_2_props)
+          apply auto[1]
+          sorry
+
+
+        then show ?thesis
+          
+      qed
+
+    qed
+  qed
+
+qed
+
+
+lemma invar_dist'_holds_upd1[invar_holds_intros]: 
+  "\<lbrakk>BFS_call_1_conds bfs_state; invar_1 bfs_state; invar_2 bfs_state; invar_3_1 bfs_state;
+    invar_3_2 bfs_state; invar_3_4 bfs_state; invar_dist' bfs_state\<rbrakk> 
+    \<Longrightarrow> invar_dist' (BFS_upd1 bfs_state)"
+proof(intro invar_props_intros, goal_cases)
+  define bfs_state' where "bfs_state' \<equiv> BFS_upd1 bfs_state"
+  let ?dSrcsG = "distance_set (Graph.digraph_abs G) (t_set srcs)"
+  let ?dSrcsT = "distance_set (Graph.digraph_abs (parents bfs_state)) (t_set srcs)"
+  let ?dSrcsT' = "distance_set (Graph.digraph_abs (parents bfs_state')) (t_set srcs)"
+  let ?dCurrG = "distance_set (Graph.digraph_abs G)  (t_set (current bfs_state))"
+  case (1 v)
+  then show ?case
+  proof(cases "distance_set (Graph.digraph_abs G) (t_set srcs) v = \<infinity>")
+    case infinite: True
+    moreover have "?dSrcsG v \<le> ?dSrcsT' v"
+      using \<open>invar_1 bfs_state\<close> \<open>invar_2 bfs_state\<close>
+      by(fastforce simp: bfs_state'_def BFS_upd1_def Let_def intro: distance_set_subset)    
+    ultimately show ?thesis
+      by (simp add: bfs_state'_def)
+  next
+    case finite: False
+    show ?thesis
+    proof(cases "v \<in> t_set (visited bfs_state)")
+      case v_in_tree: True
+      hence "?dSrcsT v = ?dSrcsG v"
+        using \<open>invar_dist' bfs_state\<close> \<open>invar_1 bfs_state\<close> \<open>invar_2 bfs_state\<close> \<open>v \<in> dVs (Graph.digraph_abs G)\<close>
+        by (auto elim!: invar_dist'_props invar_1_props invar_2_props)
+
+      moreover have "?dSrcsT v = ?dSrcsT' v"
+      proof-
+        have "?dSrcsT' v \<le> ?dSrcsT v"
+          using \<open>invar_1 bfs_state\<close>
+          by(fastforce simp: bfs_state'_def BFS_upd1_def Let_def intro: distance_set_subset)
+
+        moreover have "?dSrcsG v \<le> ?dSrcsT' v"
+          using \<open>invar_1 bfs_state\<close> \<open>invar_2 bfs_state\<close>
+          by(fastforce simp: bfs_state'_def BFS_upd1_def Let_def intro: distance_set_subset)
+
+        ultimately show ?thesis
+          using \<open>?dSrcsT v = ?dSrcsG v\<close>
+          by auto
+      qed
+      ultimately show ?thesis
+        by (auto simp: bfs_state'_def)
+    next
+      case v_not_in_tree: False
+
+
+      show ?thesis
+      proof(rule ccontr, goal_cases)
+        case 1
+        moreover have \<open>invar_2 bfs_state'\<close>
+          using \<open>BFS_call_1_conds bfs_state\<close> \<open>invar_1 bfs_state\<close> \<open>invar_2 bfs_state\<close>
+          by (auto intro!: invar_2_holds_upd1 simp: bfs_state'_def)
+        hence \<open>Graph.digraph_abs (parents bfs_state') \<subseteq> Graph.digraph_abs G\<close>
+          by auto
+        ultimately have "?dSrcsG v < ?dSrcsT' v"
+          by (simp add: distance_set_subset order_less_le bfs_state'_def)
+        hence "?dSrcsG v < ?dSrcsT' v"
+          text \<open>because the tree is a subset of the Graph, which invar?\<close>
+          by (simp add: distance_set_subset order_less_le bfs_state'_def)
+
+        have "v \<in> t_set (current (BFS_upd1 bfs_state))"
+          using \<open>v \<in> t_set (visited (BFS_upd1 bfs_state))\<close> v_not_in_tree \<open>invar_1 bfs_state\<close>
+          by (auto simp: BFS_upd1_def Let_def)
+        moreover then  obtain v' where v'[intro]: 
+          "v \<in> neighbourhood (Graph.digraph_abs G) v'" "v' \<in> t_set (current bfs_state)"
+          "v \<in> neighbourhood (Graph.digraph_abs (parents bfs_state')) v'" 
+          using v_not_in_tree \<open>invar_1 bfs_state\<close>
+          by (auto simp: neighbourhoodD BFS_upd1_def Let_def bfs_state'_def elim!: invar_1_props)
+        ultimately have "?dSrcsG v = ?dSrcsG v' + 1"
+          using \<open>invar_1 bfs_state\<close> \<open>invar_3_4 bfs_state\<close>
+          by (auto intro!: dist_current_plus_1)
+        also have "... = ?dSrcsT v' + 1"
+          text \<open>From this current invariant\<close>
+          using \<open>invar_dist' bfs_state\<close> \<open>v' \<in> t_set (current bfs_state)\<close> \<open>invar_1 bfs_state\<close>
+                \<open>invar_2 bfs_state\<close> 
+          by (force elim!: invar_1_props invar_2_props invar_dist'_props)
+        also have "... = ?dSrcsT' v' + 1"
+        proof-
+          have "?dSrcsT v' = ?dSrcsT' v'"
+          proof-
+            have "?dSrcsT' v' \<le> ?dSrcsT v'"
+              using \<open>invar_1 bfs_state\<close>
+              by(fastforce simp: bfs_state'_def BFS_upd1_def Let_def intro: distance_set_subset)
+
+            moreover have "?dSrcsG v' \<le> ?dSrcsT' v'"
+              using \<open>invar_1 bfs_state\<close> \<open>invar_2 bfs_state\<close>
+              by(fastforce simp: bfs_state'_def BFS_upd1_def Let_def intro: distance_set_subset)
+            moreover have \<open>?dSrcsT v' = ?dSrcsG v'\<close>
+              using \<open>invar_dist' bfs_state\<close> \<open>v' \<in> t_set (current bfs_state)\<close> \<open>invar_1 bfs_state\<close>
+                \<open>invar_2 bfs_state\<close> 
+              by (force elim!: invar_1_props invar_2_props invar_dist'_props)
+            ultimately show ?thesis
+              by auto
+          qed
+          then show ?thesis
+            by auto
+        qed
+        finally have "?dSrcsG v = ?dSrcsT' v' + 1"
+          by auto
+        hence "?dSrcsT' v' + 1 < ?dSrcsT' v"
+          using \<open>?dSrcsG v < ?dSrcsT' v\<close>
+          by auto
+        moreover have "v \<in> neighbourhood (Graph.digraph_abs (parents bfs_state')) v'"
+          using \<open>v \<in> neighbourhood (Graph.digraph_abs (parents bfs_state')) v'\<close> .
+        hence "?dSrcsT' v \<le> ?dSrcsT' v' + 1"
+          by (auto intro!: distance_set_neighbourhood)
+
+        ultimately show False
+          text \<open>From the triangle ineq\<close>
+          by auto
+      qed
+    qed
+  qed
+qed
+
+definition "invar_forest bfs_state \<equiv> forest (Graph.digraph_abs (parents bfs_state))"
+
+lemma invar_forest_props[elim]: 
+  "invar_forest bfs_state \<Longrightarrow> 
+  (forest (Graph.digraph_abs (parents bfs_state)) \<Longrightarrow> P)
+     \<Longrightarrow> P"
+  by (auto simp: invar_forest_def)
+
+lemma invar_forest_intro[invar_props_intros]:
+   "\<lbrakk>forest (Graph.digraph_abs (parents bfs_state))\<rbrakk>
+     \<Longrightarrow> invar_forest bfs_state"
+  by (auto simp: invar_forest_def)
+
+lemma invar_forest_holds_upd1[invar_holds_intros]: 
+  "\<lbrakk>BFS_call_1_conds bfs_state; invar_1 bfs_state; invar_2 bfs_state; invar_forest bfs_state\<rbrakk> \<Longrightarrow> invar_forest (BFS_upd1 bfs_state)"
+  apply(auto elim!: call_cond_elims invar_1_props invar_2_props invar_forest_props intro!: invar_props_intros simp: BFS_upd1_def Let_def)
+  apply(auto simp: dVs_def)
+  done
+
+lemma invar_forest_holds_4[invar_holds_intros]:
+  "\<lbrakk>BFS_ret_1_conds bfs_state; invar_forest bfs_state\<rbrakk> \<Longrightarrow> invar_forest (BFS_ret1 bfs_state)"
+  by (auto simp: intro: invar_props_intros)
+
+lemma invar_forest_holds: 
+   assumes "BFS_dom bfs_state" "invar_1 bfs_state" "invar_2 bfs_state" "invar_forest bfs_state"
+   shows "invar_forest (BFS bfs_state)"
   using assms(2-)
 proof(induction rule: BFS_induct[OF assms(1)])
   case IH: (1 bfs_state)
@@ -386,157 +1485,97 @@ proof(induction rule: BFS_induct[OF assms(1)])
 qed
 
 
-\<comment> \<open>Example of funciton package bad ind ppcl?\<close>
 
-definition "invar_3 dfs_state = (\<forall>v \<in> t_set (visited dfs_state). (\<nexists>p. Vwalk.vwalk_bet Graph.digraph_abs v p t) )"
 
-lemma invar_3_props[elim!]: "invar_3 dfs_state \<Longrightarrow> (\<lbrakk>\<And>v p. v \<in> t_set (visited dfs_state) \<Longrightarrow> \<not> (Vwalk.vwalk_bet Graph.digraph_abs v p t)\<rbrakk> \<Longrightarrow> P) \<Longrightarrow> P "
+
+definition "invar_3 bfs_state \<equiv> 
+  (\<forall>v \<in> t_set (visited bfs_state).
+       distance_set (Graph.digraph_abs (parents bfs_state)) (t_set srcs) v \<le> 
+         distance_set (Graph.digraph_abs G) (t_set srcs) v)"
+
+lemma invar_3_props[elim]: 
+  "invar_3 bfs_state \<Longrightarrow> 
+  (\<lbrakk>\<And>v. v \<in> t_set (visited bfs_state) \<Longrightarrow> 
+    distance_set (Graph.digraph_abs (parents bfs_state)) (t_set srcs) v \<le> 
+         distance_set (Graph.digraph_abs G) (t_set srcs) v\<rbrakk> \<Longrightarrow> P)
+     \<Longrightarrow> P"
   by (auto simp: invar_3_def)
 
-lemma invar_3_intro[invar_props_intros]: "\<lbrakk>\<And>v p. v \<in> t_set (visited dfs_state) \<Longrightarrow>  \<not> (Vwalk.vwalk_bet Graph.digraph_abs v p t)\<rbrakk> \<Longrightarrow> invar_3 dfs_state"
+lemma invar_3_intro[invar_props_intros]:
+   "(\<And>v. v \<in> t_set (visited bfs_state) \<Longrightarrow> 
+    distance_set (Graph.digraph_abs (parents bfs_state)) (t_set srcs) v \<le> 
+         distance_set (Graph.digraph_abs G) (t_set srcs) v)
+     \<Longrightarrow> invar_3 bfs_state"
   by (auto simp: invar_3_def)
 
-lemma invar_3_holds_1[invar_holds_intros]:
-  "\<lbrakk>DFS_call_1_conds dfs_state; invar_3 dfs_state\<rbrakk> \<Longrightarrow> invar_3 (DFS_upd1 dfs_state)"
-  by (auto simp: DFS_upd1_def dest!: append_vwalk_pref intro!: invar_props_intros)
+lemma invar_3_4_holds_upd1[invar_holds_intros]: 
+  "\<lbrakk>BFS_call_1_conds bfs_state; invar_1 bfs_state; invar_2 bfs_state ;
+    invar_3_1 bfs_state; invar_3_3 bfs_state; invar_3_4 bfs_state; invar_3 bfs_state\<rbrakk> 
+    \<Longrightarrow> invar_3 (BFS_upd1 bfs_state)"
+proof(intro invar_props_intros, goal_cases)
+  case (1 v)
+  have ?case (is "?dT'v \<le> ?dGv")
+    if "v \<notin> t_set (visited bfs_state)"
+  proof-
+    from 1 and that obtain v' where v'[intro]:
+      "v \<in> neighbourhood (Graph.digraph_abs G) v'"
+      "v' \<in> t_set (current bfs_state)" 
+      "v \<in> neighbourhood (Graph.digraph_abs (parents (BFS_upd1 bfs_state))) v'"
+      apply (auto simp: BFS_upd1_def Let_def elim!: invar_1_props invar_2_props)
+      by (simp add: neighbourhoodD)
+    hence "v' \<in> t_set (visited bfs_state)"
+      using \<open>invar_1 bfs_state\<close> \<open>invar_2 bfs_state\<close>
+      by (auto elim!: invar_1_props invar_2_props)
+    hence "distance_set (Graph.digraph_abs (parents bfs_state)) (t_set srcs) v'
+         \<le> distance_set (Graph.digraph_abs G) (t_set srcs) v'" (is "?dTv' \<le> ?dGv'")
+      using \<open>invar_3 bfs_state\<close>
+      by (auto elim!: invar_3_props)
+    moreover have "distance_set (Graph.digraph_abs (parents (BFS_upd1 bfs_state))) (t_set srcs) v'
+         \<le> ?dTv'" (is "?dT'v' \<le> _ ")
+      using \<open>invar_1 bfs_state\<close> \<open>invar_2 bfs_state\<close>
+      by (auto simp: BFS_upd1_def Let_def
+          elim!: invar_1_props invar_2_props intro!: distance_set_subset)
+    ultimately have "?dT'v' \<le> ?dGv'"
+      by auto
+    moreover have "v \<in> t_set (current (BFS_upd1 bfs_state))"
+      using 1 \<open>v \<notin> t_set (visited bfs_state)\<close>
+      by (auto si mp: BFS_upd1_def Let_def)
+    hence "?dGv = ?dGv' + 1"
+      using 1
+      by (auto intro!: dist_current_plus_1)
+    moreover have "?dT'v = ?dT'v' + 1"
+    proof-
+      have False if "?dT'v > ?dT'v' + 1"
+        using distance_set_1[OF v'(3)] that
 
-lemma invar_3_holds_2[invar_holds_intros]: "\<lbrakk>DFS_call_2_conds dfs_state; invar_1 dfs_state; invar_3 dfs_state\<rbrakk> \<Longrightarrow> invar_3 (DFS_upd2 dfs_state)"
-  by (force simp: DFS_upd2_def dest!: append_vwalk_pref intro!: invar_props_intros elim!: DFS_call_2_conds)
+        
+        by (metis add_0_left distance_set_ge_1E' distance_set_subset eSuc_plus_1 emptyE empty_subsetI ileI1 neighbourhoodI not_iless0 order_le_imp_less_or_eq zero_order(1))
+        by (simp add: leD)
+      moreover have False if "?dT'v < ?dT'v' + 1"
+      proof-
+        have "?dT'v \<le> ?dT'v'"
+          using that eSuc_plus_1 ileI1
+          by force
+        moreover have "v \<notin> t_set (visited bfs_state)"
+          using \<open>v \<notin> t_set (visited bfs_state)\<close>
+          .
 
-lemma invar_3_holds_4[invar_holds_intros]: "\<lbrakk>DFS_ret_1_conds dfs_state; invar_3 dfs_state\<rbrakk> \<Longrightarrow> invar_3 (DFS_ret1 dfs_state)"
-  by (auto simp: intro: invar_props_intros)
+        ultimately show False
+          using \<open>invar_3_4 bfs_state\<close> \<open>v' \<in> t_set (current bfs_state)\<close>
+          apply(auto elim!: invar_3_4_props)
+          sorry
+      qed
+      ultimately show ?thesis
+        by force
+    qed
+    ultimately show ?thesis
+      by auto
+  qed
 
-lemma invar_3_holds_5[invar_holds_intros]: "\<lbrakk>DFS_ret_2_conds dfs_state; invar_3 dfs_state\<rbrakk> \<Longrightarrow> invar_3 (DFS_ret2 dfs_state)"
-  by (auto simp: intro: invar_props_intros)
+  oops
 
-lemma invar_3_holds: 
-   assumes "DFS_dom dfs_state" "invar_1 dfs_state" "invar_3 dfs_state"
-   shows "invar_3 (DFS dfs_state)" 
-   using assms(2-)
-proof(induction rule: DFS_induct[OF assms(1)])
-  case IH: (1 dfs_state)
-  show ?case
-    apply(rule DFS_cases[where dfs_state = dfs_state])
-    by (auto intro!: IH(2-5) invar_holds_intros simp: DFS_simps[OF IH(1)])
-qed
 
-abbreviation "seen_verts dfs_state \<equiv> (set (stack dfs_state) \<union> t_set (visited dfs_state))"
 
-definition "state_rel_1 dfs_state_1 dfs_state_2 
-              \<equiv> seen_verts dfs_state_1 \<subseteq> seen_verts dfs_state_2"
-
-lemma state_rel_1_props[elim!]: "state_rel_1 dfs_state_1 dfs_state_2 \<Longrightarrow>
-                                  (seen_verts dfs_state_1 \<subseteq> seen_verts dfs_state_2 \<Longrightarrow> P) \<Longrightarrow> P "
-  by (auto simp: state_rel_1_def)
-
-lemma state_rel_1_intro[state_rel_intros]: "\<lbrakk>seen_verts dfs_state_1 \<subseteq> seen_verts dfs_state_2\<rbrakk> \<Longrightarrow> state_rel_1 dfs_state_1 dfs_state_2"
-  by (auto simp: state_rel_1_def)
-
-lemma state_rel_1_trans:
-  "\<lbrakk>state_rel_1 dfs_state_1 dfs_state_2; state_rel_1 dfs_state_2 dfs_state_3\<rbrakk> \<Longrightarrow>
-   state_rel_1 dfs_state_1 dfs_state_3"
-  by (auto intro!: state_rel_intros)
-
-lemma state_rel_1_holds_1[state_rel_holds_intros]:
-  "\<lbrakk>DFS_call_1_conds dfs_state\<rbrakk> \<Longrightarrow> state_rel_1 dfs_state (DFS_upd1 dfs_state)"
-  by (auto simp: DFS_upd1_def intro!: state_rel_intros)
-
-lemma state_rel_1_holds_2[state_rel_holds_intros]:
-  "\<lbrakk>DFS_call_2_conds dfs_state; invar_1 dfs_state\<rbrakk> \<Longrightarrow> state_rel_1 dfs_state (DFS_upd2 dfs_state)"
-  by (auto simp: DFS_upd2_def intro!: state_rel_intros elim: call_cond_elims)
-
-lemma state_rel_1_holds_4[state_rel_holds_intros]:
-  "\<lbrakk>DFS_ret_1_conds dfs_state\<rbrakk> \<Longrightarrow> state_rel_1 dfs_state (DFS_ret1 dfs_state)"
-  by (auto simp: intro!: state_rel_intros)
-
-lemma state_rel_1_holds_5[state_rel_holds_intros]:
-  "\<lbrakk>DFS_ret_2_conds dfs_state\<rbrakk> \<Longrightarrow> state_rel_1 dfs_state (DFS_ret2 dfs_state)"
-  by (auto simp: intro!: state_rel_intros)
-
-lemma state_rel_1_holds: 
-   assumes "DFS_dom dfs_state" "invar_1 dfs_state"
-   shows "state_rel_1 dfs_state (DFS dfs_state)" 
-   using assms(2-)
-proof(induction rule: DFS_induct[OF assms(1)])
-  case IH: (1 dfs_state)
-  show ?case
-    apply(rule DFS_cases[where dfs_state = dfs_state])
-    by (auto intro: state_rel_1_trans invar_holds_intros state_rel_holds_intros intro!: IH(2-) simp: DFS_simps[OF IH(1)])
-qed
-
-definition "state_rel_2 dfs_state_1 dfs_state_2 
-              \<equiv> (\<forall>v \<in> set (stack dfs_state_1). ((\<exists>p. Vwalk.vwalk_bet Graph.digraph_abs v p t) \<or> v = t) \<longrightarrow> v \<in> set (stack dfs_state_2))"
-
-lemma state_rel_2_props[elim!]: "state_rel_2 dfs_state_1 dfs_state_2 \<Longrightarrow>
-                                  \<lbrakk>\<lbrakk>\<And>v.\<lbrakk>v \<in> set (stack dfs_state_1); (\<exists>p. Vwalk.vwalk_bet Graph.digraph_abs v p t) \<or> v = t\<rbrakk>
-                                    \<Longrightarrow> v \<in> set (stack dfs_state_2)\<rbrakk> \<Longrightarrow> P\<rbrakk> \<Longrightarrow> P "
-  by (auto simp: state_rel_2_def)
-
-lemma state_rel_2_intro[state_rel_intros]: "\<lbrakk>\<And>v. \<lbrakk>v \<in> set (stack dfs_state_1); (\<exists>p. Vwalk.vwalk_bet Graph.digraph_abs v p t) \<or> v = t\<rbrakk>
-                                    \<Longrightarrow> v \<in> set (stack dfs_state_2)\<rbrakk> \<Longrightarrow> state_rel_2 dfs_state_1 dfs_state_2"
-  by (auto simp: state_rel_2_def)
-
-lemma state_rel_2_trans:
-  "\<lbrakk>state_rel_2 dfs_state_1 dfs_state_2; state_rel_2 dfs_state_2 dfs_state_3\<rbrakk> \<Longrightarrow>
-   state_rel_2 dfs_state_1 dfs_state_3"
-  by (auto intro!: state_rel_intros)
-
-lemma state_rel_2_holds_1[state_rel_holds_intros]:
-  "\<lbrakk>DFS_call_1_conds dfs_state\<rbrakk> \<Longrightarrow> state_rel_2 dfs_state (DFS_upd1 dfs_state)"
-  by (auto simp: DFS_upd1_def intro!: state_rel_intros)
-
-lemma state_rel_2_holds_2[state_rel_holds_intros]:
-  "\<lbrakk>DFS_call_2_conds dfs_state; invar_1 dfs_state; invar_3 dfs_state\<rbrakk> \<Longrightarrow> state_rel_2 dfs_state (DFS_upd2 dfs_state)"
-  by (force simp: DFS_upd2_def intro!: state_rel_intros elim!: DFS_call_2_conds)
-
-lemma state_rel_2_holds_4[state_rel_holds_intros]:
-  "\<lbrakk>DFS_ret_1_conds dfs_state\<rbrakk> \<Longrightarrow> state_rel_2 dfs_state (DFS_ret1 dfs_state)"
-  by (auto simp: intro!: state_rel_intros)
-
-lemma state_rel_2_holds_5[state_rel_holds_intros]:
-  "\<lbrakk>DFS_ret_2_conds dfs_state\<rbrakk> \<Longrightarrow> state_rel_2 dfs_state (DFS_ret2 dfs_state)"
-  by (auto simp: intro!: state_rel_intros)
-
-lemma state_rel_2_holds: 
-   assumes "DFS_dom dfs_state" "invar_1 dfs_state" "invar_3 dfs_state"
-   shows "state_rel_2 dfs_state (DFS dfs_state)" 
-   using assms(2-)
-proof(induction rule: DFS_induct[OF assms(1)])
-  case IH: (1 dfs_state)
-  show ?case
-    apply(rule DFS_cases[where dfs_state = dfs_state])
-    by (auto intro: state_rel_2_trans invar_holds_intros state_rel_holds_intros intro!: IH(2-) simp: DFS_simps[OF IH(1)])
-qed
-
-lemma DFS_ret_1[ret_holds_intros]: "DFS_ret_1_conds (dfs_state) \<Longrightarrow> DFS_ret_1_conds (DFS_ret1 dfs_state)"
-  by (auto simp: elim!: call_cond_elims intro!: call_cond_intros)
-
-lemma ret1_holds:
-   assumes "DFS_dom dfs_state" "return (DFS dfs_state) = NotReachable"
-   shows "DFS_ret_1_conds (DFS dfs_state)" 
-   using assms(2-)
-proof(induction  rule: DFS_induct[OF assms(1)])
-  case IH: (1 dfs_state)
-  show ?case
-    apply(rule DFS_cases[where dfs_state = dfs_state])
-    using IH(4)                                                                
-    by (auto intro: ret_holds_intros intro!: IH(2-) simp: DFS_simps[OF IH(1)])
-qed
-
-lemma DFS_ret_2[ret_holds_intros]: "DFS_ret_2_conds (dfs_state) \<Longrightarrow> DFS_ret_2_conds (DFS_ret2 dfs_state)"
-  by (auto simp: elim!: call_cond_elims intro!: call_cond_intros)
-
-lemma ret2_holds:
-   assumes "DFS_dom dfs_state" "return (DFS dfs_state) = Reachable"
-   shows "DFS_ret_2_conds (DFS dfs_state)" 
-   using assms(2-)
-proof(induction  rule: DFS_induct[OF assms(1)])
-  case IH: (1 dfs_state)
-  show ?case
-    apply(rule DFS_cases[where dfs_state = dfs_state])
-    using IH(4)                                                                
-    by (auto intro: ret_holds_intros intro!: IH(2-) simp: DFS_simps[OF IH(1)])
-qed
 
 end
                                                                
