Pair_Graph/Tree_Defs.thy
@@ -1,0 +1,13 @@
+theory Tree_Defs
+  imports Pair_Graph
+begin
+
+locale tree =
+fixes
+  root :: 'a
+assumes
+  root_in_T: "root \<in> dVs T" and
+  unique_awalk: "v \<in> dVs T \<Longrightarrow> \<exists>!p. Vwalk.vwalk root p v"
+begin
+
+end
